# Congruences
## Definition
Let $a, b \in \mathbb Z$, and let $m \in \mathbb Z^+$. The integers $a$ and $b$ are *congruent modulo $m$*, written $a \equiv b \mod m$, if $m \mid (a - b)$.

## Theorem
Let $a_1, b_1, a_2, b_2 \in \mathbb Z$, $m \in \mathbb Z^+$. Assume $a_1 \equiv a_2 \mid m$, $b_1 \equiv b_2 \mod m$. Then,
1. $a_1 + b_1 \equiv a_2 + b_2 \mod m$
2. $a_1 - b_1 \equiv a_2 - b_2 \mod m$
3. $a_1 + c \equiv a_2 + c \mod m$
4. $a_1 b_1 \equiv a_2 b_2 \mod m$
5. $a_1 c \equiv a_2 c \mod m$

### Some Proofs
1. Assume $a_1 \equiv a_2 \mod m$, $b_1 \equiv b_2 \mod m$.
 - We may fix $s \in \mathbb Z$ such that $a_1 - a_2 = ms$
 - Similarily, fix $t \in \mathbb Z$ such that $b_1 - b_2 = mt$.
  - observe that 
   $$\begin{align*}
	    m(s + t) = ms + mt 
		    &= (a_1 - a_2) + (b_1 - b_2) \\
		    &= (a_1 + b_1) - (a_2 + b_2)
    \end{align*}$$
 - Thus by the definition of congruence $\mod m$, $a_1 + b_1 \equiv a_2 + b_2 \mod m$.
  
3. Assume $a_1 \equiv a_2 \mod m$.
 - Let $c \in \mathbb Z$. We proved that $c \equiv c \mod m$ (by reflexivity).
 - By part *1)*, $a_1 + c \equiv a_2 + c \mod m$.
  
4. Assume $a_1 \equiv a_2 \mod m$ and $b_1 \equiv b_2 \mod m$.
 - We fix $s \in \mathbb Z$ such that $a_1 - a_2 = ms$.
 - We fix $t \in \mathbb Z$ such that $b_1 - b_2 = mt$.
 - $$\begin{align*}
		a_1 b_1 - a_2 b_2
		&=
			a_1 b_1 - a_1 b_2 + a_1 b_2 - a_2 b_2
		\\&=
			a_1 (b_1 - b_2) + b_2 (a_1 - a_2)
		\\&=
			a_1 (mt) + b_2 (ms)
		\\&=
			m(a_1 t + b_2 s)
  \end{align*}$$
 - so $m \mid a_1 b_1 - a_2 b_2$ i.e. $a_1 b_1 \equiv a_2 b_2 \mod m$