# 1 - 1.2f)
$y + y \cdot x +y \cdot x \cdot z$

# 2 - 1.4)
Suppose $E[z:=X]=E[z:=Y]$ is true in every state for every expression $E$. Then, $E : z$  would be such a valid expression, such that $E[z:=X]=E[z:=Y] \equiv z[z:=X]=z[z:=Y] \equiv X = Y$ . So $X = Y$ is true in every state.

# 3 - 1.7e)
1. $E: z \cdot x + z \cdot y;$ 
    $E[z := y+1] = (y+1) \cdot x + (y + 1) \cdot y$
2. $E: 7 \cdot x + 7 \cdot y$
    $E[z := y+1] = 7 \cdot x + 7 \cdot y$ 
3. $E: z \cdot x + 7 \cdot y$
    $E[z := y+1] = (y + 1) \cdot x + 7 \cdot y$
4. $E: 7 \cdot x + z \cdot y$
    $E[z := y+1] = 7 \cdot x + (y + 1) \cdot y$

# 4 - 1.9a)
$E: (x + y) \cdot z$, $X = Y \equiv x + y = y + x$

# 5 - 1.11e)
*Precondition:* $\{(y = x+y)[y := x+y]\} \equiv \{x + y = x + x + y\}$ 
*Postcondition:* $\{y = x+y\}$

# 6 - 2.1)
|Question|$S_0$ Answer|$S_1$ Answer|
|-|-|-|
|k|t|t|
|l|t|t|
|m|f|t|

# 7 - 2.2)
## g)
| $b$ | $c$ | $\neg b$ | $\neg b \equiv c$ | $(\neg b \equiv c) \lor b$ |
| :-: | :-: | :-: | :-: | :-: |
| T | T | F | F | T |
| T | F | F | T | T |
| F | T | T | T | T |
| F | F | T | F | F |

## h)
| $b$ | $c$ | $b \equiv c$ | $b \Rightarrow c$ | $c \Rightarrow b$ | $(b \Rightarrow c) \land (c \Rightarrow b)$ | $(b \equiv c) \equiv (b \Rightarrow c) \land (c \Rightarrow b)$ |
| :-: | :-: | :-: | :-: | :-: | :-: | :-: |
| T | T | T | T | T | T | T |
| T | F | F | F | T | F | T |
| F | T | F | T | F | F | T |
| F | F | T | T | T | T | T |

 # 8 - 2.3)
 ## f)
$$\begin{align*}
	(\lnot b \Leftarrow b \lor c)_D
	&= \lnot b \not \Rightarrow b \land c
\end{align*}$$
| $b$ | $c$ | $\neg b$ | $b \land c$ | $\neg b \not \Rightarrow b \land c$ |
| :-: | :-: | :-: | :-: | :-: |
| T | T | F | T | F |
| T | F | F | F | F |
| F | T | T | F | T |
| F | F | T | F | T |

## g)
$$\begin{align*}
	((\lnot b \equiv true) \lor b)_D
	&= (\lnot b \not \equiv false) \land b
\end{align*}$$
| $b$ | $\neg b$ | $\neg b \not \equiv False$ | $(\neg b \not \equiv False) \land b$ |
| :-: | :-: | :-: | :-: |
| T | F | F | F |
| F | T | T | F |

# 9 - 2.5)
## d)
Let $C$ be the statement "it's raining cats" and let $D$ be the statement "It's raining dogs". Then, the boolean expression is $C \lor D$

## e)
Let 
- $C$ be "it's raining cats", 
- $D$ be "it's raining dogs"
- $H$ be "I'll eat my hat"
- $S$ be "I'll go swimming"

Then the boolean expression is
$$C \lor D \Rightarrow H \land \lnot S$$

# 10 - 2.7) ***TODO***
## h)


## i)

## j)

# 11 - 2.9) ***TODO***
Let
- $B$ be the statement "Bill takes the bus"
- $A$ be "Bill makes his appointment"
- $L$ be "The bus is late"
- $H$ be "Bill should go home"
- $D$ be "Bill feels downcast"
- $J$ be "Bill gets a job"

Then, the three assumptions can be described as follows:

> [!NOTE] Three Assumptions
> 1. $B \Rightarrow L \Rightarrow \lnot A$
> 2. $\lnot A \land D \Rightarrow \lnot H$
> 3. $\lnot J \Rightarrow D \land \lnot H$

## 8 Conjectures
4. $B \Rightarrow L \Rightarrow J$
5. $\lnot A \land H \Rightarrow J$
6. $L \land D \land H \Rightarrow \lnot B$
7. $L \land \lnot J \Rightarrow \lnot B$
8. $A \Rightarrow \lnot H \land \lnot J$
9. $\lnot B \lor \lnot A \Rightarrow D$
10. $B \land L \land H \Rightarrow J$
11. $B \land \lnot J \Rightarrow (B \not \Leftrightarrow \lnot H)$

# 12 - 2.10) ***TODO***

# 13)
## Prove Existence
In boolean algebra, every element $x$ must be in the set $\{true, false\}$. If $x \equiv true$ , then $\lnot x \equiv false$. Likewise, if $x \equiv false$, then $\lnot x \equiv true$. So every $x$ in boolean algebra has a complement.

## Prove Uniqueness
Suppose that $x$ has arbitrary complements $x_1$ and $x_2$. Then, given $x \lor \lnot x \equiv true$ and $x \land \lnot x \equiv false$, we have
$$\begin{align*}
	x \lor x_1 &\equiv x \lor x_2 \\
	(x \lor x_1) \land x_1 &\equiv (x \lor x_2) \land x_1 \\
	x \land x_1 \lor x_1 \land x_1
	&\equiv
		x \land x_1 \lor x_2 \land x_1 \\
	x_1 &\equiv x_2 \land x_1
\end{align*}$$
Similarly,
$$\begin{align*}
	x \lor x_1 &\equiv x \lor x_2 \\
	(x \lor x_1) \land x_2 &\equiv (x \lor x_2) \land x_2 \\
	x \land x_2 \lor x_1 \land x_2
	&\equiv
		x \land x_2 \lor x_2 \land x_2 \\
	x_1 \land x_2  &\equiv x_2
\end{align*}$$
Thus we have $x_1 \equiv x_2 \land x_1 \equiv x_1 \land x_2 \equiv x_2$, so by the inference rule of transitivity, we have that $x_1 \equiv x_2$, so the complement of $x$ is unique.

# 14)
List all the combinations such that $f(x, y, z) \equiv f(\lnot x, \lnot y, \lnot z)$
$f(x, y, z)$|$f(\lnot x, \lnot y, \lnot z)$
:-:|:-:
f(0,0,0)|f(1,1,1)
f(0,0,1)|f(1,1,0)
f(0,1,0)|f(1,0,1)
f(0,1,1)|f(1,0,0)
f(1,0,0)|f(0,1,1)
f(1,0,1)|f(0,1,0)
f(1,1,0)|f(0,0,1)
f(1,1,1)|f(0,0,0)

> [!NOTE] Notice
> Symmetrical combinations such as $f(0, 0, 0), f(1, 1, 1)$ and $f(1,1,1), f(0, 0, 0)$ give the same proposition, so we can remove them.

$f(x, y, z)$|$f(\lnot x, \lnot y, \lnot z)$
:-:|:-:
f(0,0,0)|f(1,1,1)
f(0,0,1)|f(1,1,0)
f(0,1,0)|f(1,0,1)
f(0,1,1)|f(1,0,0)

In each of these 4 cases, there are 2 return values for the function. 

$\therefore$ there are $2^4 = 16$ boolean functions

# 15 - 3.4)
## Prove $(\Rightarrow)$
Suppose that $Q \equiv true$ is a theorem. We prove that $Q$ is a theorem.
$$\begin{align*}
	&Q \\
	&Q \equiv true \tag{Identity: $(true \equiv Q) \equiv Q$}
\end{align*}$$
$\therefore$ $Q$ is a theorem.

## Prove ($\Leftarrow$)
Suppose that $Q$ is a theorem. We prove that $Q \equiv true$ is a theorem.
$$\begin{align*}
	Q &\equiv true \\
	true &\equiv Q \tag{Symmetry} \\
	&Q \tag{Identity: $(true \equiv Q) \equiv Q$}
\end{align*}$$

# 16 - 3.6)
![[Pasted image 20220920181008.png]]

> [!NOTE] Definitions
> Define $\oplus$ to be the first prefix operator and $\triangle$ to be the last prefix operator. 

### Case $\oplus$:
We have that $\oplus true \equiv true \not \equiv false$, so by transitivity $\oplus true \not \equiv false$ thus $\oplus$ does not satisfy  the axioms.

### Case $id$:
We have that $\oplus id \equiv true \not \equiv false$, so by transitivity $\oplus id \not \equiv false$ thus $id$ does not satisfy  the axioms.

### Case $\triangle$:
$\triangle true \equiv false$, thus $\triangle$ satisfies axiom (3.8)

$$\begin{align*}
	\triangle(p \equiv q)\ &\equiv\ false \\
	\triangle p \equiv q\ &\equiv\ false \equiv q
\end{align*}$$
But we have that when $q \equiv false$, then $\triangle p \equiv q\ \equiv\ true \not \equiv false \equiv \triangle(p \equiv q)$, so by transitivity $\triangle p \equiv q \ \not \equiv \ \triangle(p \equiv q)$, thus axiom (3.9) fails.

### Case $\lnot$:
$\lnot true \equiv false$, thus $\lnot$ satisfies axiom (3.8)

$$\begin{align*}
	\lnot(p \equiv q)
	&\equiv
		\lnot((p \Rightarrow q) \land (q \Rightarrow p))
	\\&\equiv
		\lnot((\lnot p \lor q) \land (\lnot q \lor p))
	\\&\equiv
		\lnot(\lnot p \lor q) \lor \lnot (\lnot q \lor p)
	\\&\equiv
		(p \land \lnot q) \lor (q \land \lnot p)
	\\&\equiv
		(p \land \lnot q \lor q) \land (p \land \lnot q \lor\lnot p)
	\\&\equiv
		(p \lor q) \land (\lnot q \lor\lnot p)
	\\&\equiv
		(\lnot p \Rightarrow q) \land (q \Rightarrow \lnot p)
	\\&\equiv
		\lnot p \equiv q
\end{align*}$$
$\therefore$ axiom (3.9) holds for $\lnot$.

# 17 - 3.12)
$$\begin{align*}
	((p \not \equiv q) \not \equiv r)
	&\equiv
		(\lnot (p \equiv q) \not \equiv r)
	\\&\equiv
		((\lnot p \equiv q) \not \equiv r)
	\\&\equiv
		((\lnot p \equiv q) \equiv \lnot r)
	\\&\equiv
		(\lnot p \equiv (q \equiv \lnot r))
	\\&\equiv
		(p \not \equiv (q \not \equiv r))
\end{align*}$$

# 18 - 3.13)
$$\begin{align*}
	((p \not \equiv q) \equiv r)
	&\equiv
		(\lnot (p \equiv q) \equiv r)
	\\&\equiv
		(\lnot p \equiv q \equiv r)
	\\&\equiv
		(\lnot p \equiv (q \equiv r))
	\\&\equiv
		(p \not \equiv (q \equiv r))
\end{align*}$$
$\therefore$ associativity of $\not \equiv$ has been proven.

# 19 - 3.17) ***TODO***
$$\begin{align*}
	p \lor false
	&\equiv
		p \lor (\lnot p \equiv p) \tag{3.15}
	\\&\equiv
		p \lor ((\lnot p \Rightarrow p) \land (p \Rightarrow \lnot p))
	\\&\equiv
		p \lor ((p \lor p) \land (\lnot p \lor \lnot p))
	\\&\equiv
		p \lor (p \land \lnot p)
	\\&\equiv \tag{(3.43) Absorption}
		p
\end{align*}$$

# 20 - 3.18)
$$\begin{align*}
	p \lor (q \lor r)
	&\equiv \tag{idempotency}
		(p \lor p) \lor (q \lor r)
	\\&\equiv \tag{associativity}
		p \lor (p \lor q) \lor r
	\\&\equiv \tag{symmetry}
		p \lor (q \lor p) \lor r
	\\&\equiv \tag{associativity}
		(p \lor q) \lor (p \lor r)
\end{align*}$$

# 21 - 3.22)
$$\begin{align*}
	p \land q
	&\equiv \tag{Golden rule}
		p \equiv q \equiv p \lor q
	\\&\equiv
		p \equiv (q \Rightarrow p \lor q) \land (p \lor q \Rightarrow q)
	\\&\equiv
		p \equiv (\lnot q \lor p \lor q) \land (\lnot p \land \lnot q \lor q)
	\\&\equiv \tag{Absorbtion, Zero of $\lor$}
		p \equiv true \land (\lnot p \lor q)
	\\&\equiv \tag{Absorbtion}
		p \equiv \lnot p \lor q
	\\&\equiv
		(p \Rightarrow \lnot p \lor q) \land (\lnot p \lor q \Rightarrow p)
	\\&\equiv
		(\lnot p \lor \lnot p \lor q) \land (p \land \lnot q \lor p)
	\\&\equiv \tag{Idempodency, Absorption}
		(\lnot p \lor q) \land p
	\\&\equiv
		q \land p
\end{align*}$$

# 22 - 3.24)
$$\begin{align*}
	p \land false 
	&\equiv \tag{Golden rule; $q:=false$}
		p \equiv false \equiv p \lor false
	\\&\equiv \tag{Identity of $\lor$}
		(p \Rightarrow false) \land (false \Rightarrow p) \equiv p
	\\&\equiv
		(\lnot p \lor false) \land (true \lor p) \equiv p
	\\&\equiv \tag{Identity of $\lor$, Zero of $\land$}
		\lnot p \land true \equiv p
	\\&\equiv \tag{Identity of $\land$}
		\lnot p \equiv p
	\\&\equiv \tag{Contradiction}
		false
\end{align*}$$

# 23 - 3.32)
$$\begin{align*}
	\lnot (p \land q)
	&\equiv \tag{3.48}
		\lnot (p \land \lnot q \equiv \lnot p)
	\\&\equiv \tag{Distributivity}
		p \land \lnot q \equiv p
	\\&\equiv
		(p \Rightarrow p \land \lnot q) \land (p \land \lnot q \Rightarrow p)
	\\&\equiv
		(\lnot p \lor p \land \lnot q) \land (\lnot (p \land \lnot q) \lor p)
	\\&\equiv \tag{Absorption}
		(\lnot p \lor \lnot q) \land (\lnot (p \land \lnot q) \lor p)
	\\&\equiv \tag{(3.47b) De Morgan}
		(\lnot p \lor \lnot q) \land (\lnot p \lor q \lor p)
	\\&\equiv \tag{Zero of $\lor$}
		(\lnot p \lor \lnot q) \land true
	\\&\equiv \tag{Identity of $\land$}
		\lnot p \lor \lnot q
\end{align*}$$

# 24 - 3.34)
$$\begin{align*}
	(p \land q) \lor (p \land \lnot q)
	&\equiv \tag{Distributivity}
		p \land (q \lor \lnot q)
	\\&\equiv \tag{Excluded Middle}
		p \land true
	\\&\equiv \tag{Identity of $\land$}
		p
\end{align*}$$

# 25 - 3.43)
$$\begin{align*}
	p \Rightarrow q
	&\equiv
		\lnot p \lor q
	\\&\equiv \tag{Symmetry of $\lor$}
		q \lor \lnot p
	\\&\equiv
		\lnot q \Rightarrow \lnot p
\end{align*}$$

# 26 - 3.45)
$$\begin{align*}
	p \Rightarrow q
	&\equiv
		\lnot p \lor q
	\\&\equiv \tag{De Morgan's Law}
		\lnot (p \land \lnot q)
	\\&\equiv \tag{3.48, Symmetry}
		\lnot (p \land q \equiv \lnot p)
	\\&\equiv \tag{Distributivity}
		\lnot p \lor \lnot q \equiv \lnot p
\end{align*}$$

# 27 - 3.48)


