# Assignment #5

![[Pasted image 20220304214844.png]]
$$\begin{align*}
	\frac x {5+x^4}
	&=
		\frac x 5 \cdot \frac1 {1 + \frac{x^4}{5}} \\
	&=
		\frac x 5 \sum_{n=0}^\infty
		\left(-\frac{x^4}{5}\right)^n
	\\&=
		\sum_{n=0}^\infty
		(-1)^n \left(\frac 1 5\right)^{n+1}
		x^{4n+1}
\end{align*}$$

$$\begin{align*}
	\lim_{n\to\infty} \frac{
		\frac 1 {5^{n+2}} x^{4n+5}
	} {
		\frac 1 {5^{n+1}} x^{4n+1}
	}
	&=
		\lim_{n\to\infty} 
		\frac 1 5 x^4 < 1
	\\&=
		x^4 < 5
	\\&\equiv
		x < \sqrt[4]{5}
\end{align*}$$
![[Pasted image 20220304220001.png]]
$$\begin{align*}
	\int \sum_{n=1}^\infty
	(-1)^{n-1} \frac{x^{3n}}{n}
	\ dx
	&=
		\int \sum_{n=1}^\infty
		\frac{(-1)^{n-1}x^{3n}}{n}
		\ dx
	\\&=
		\sum_{n=1}^\infty
		\frac{(-1)^{n-1}x^{3n+1}}{n(3n+1)} + c
	\\&=
		\sum_{n=0}^\infty
		\frac{(-1)^{n}x^{3n+4}}{(n+1)(3n+4)} + c
\end{align*}$$

![[Pasted image 20220304222241.png]]
$$\begin{align*}
	&= \sin(\frac \pi 6) = \frac 1 2
\end{align*}$$

![[Pasted image 20220304223400.png]]
$$\begin{align*}
	(x^{-2})' &= -2x^{-3} \\
	(x^{-2})^{(n)} &= (-1)^n (n+1)! x^{-n-2} \\
	\\
	\sum_{n=0}^\infty \frac{
		(-1)^n (n+1)! 2^{-n-2}
	} {
		n!
	} (x - 2)^n
	&=
		\sum_{n=0}^\infty \frac{
			(-1)^n (n+1)
		} {
			2^{n+2}
		} (x - 2)^n
\end{align*}$$

![[Pasted image 20220304224119.png]]
$$\begin{align*}
	\binom{\frac 1 4}{n}
	&=
		\frac{
			\tfrac 1 4 (-\tfrac 3 4) (-\tfrac 7 4)
			\cdots (\tfrac 1 4 - n + 1)
		} {
			n!
		}
	\\&=
		\frac{
			(-3) (-7) \cdots (1 - 4n + 4)
		} {
			4^n n!
		}
	\\&=
		\frac{
			(-1)^{n-1} (3) (7) \cdots (4n - 5)
		} {
			4^n n!
		}
\end{align*}$$

![[Pasted image 20220304225102.png]]
$$\begin{align*}
	\frac d {dx} (4 + xe^{3x}) \Big|_{x=0}
	&=
		e^{3x} + 3xe^{3x} \Big|_{x=0}
	&&=
		1 \\
	\frac{d^2}{dx^2} (4 + xe^{3x}) \Big|_{x=0}
	&=
		3e^{3x} + 3e^{3x} + 9xe^{3x} \Big|_{x=0}
	\\&=
		6e^{3x} + 9xe^{3x} \Big|_{x=0}
	&&=
		6
	\\
	4 +
	\frac 1 {1!} (1)^n +
	\frac 6 {2!} (1)^n
	&=
		8
\end{align*}$$

![[Pasted image 20220304231111.png]]
$$\begin{align*}
	|-6 x^{-4}| \leq 6(0.2)^{-4} = 3750
\end{align*}$$

![[Pasted image 20220304233459.png]]
$$\begin{align*}
	y' &= -\frac{
		x
	} {
		\sqrt{16 - x^2}
	}
	\\
	2 \pi \int_{-2}^3 
	\sqrt{16 - x^2} 
	\sqrt{1 + (-\tfrac{
		x
	} {
		\sqrt{16 - x^2}
	})^2} \ dx
	&=
		2 \pi \int_{-2}^3 
		\sqrt{16 - x^2} 
		\sqrt{1 + \tfrac{
			x^2
		} {
			16 - x^2
		}} \ dx
	\\&=
		2 \pi \int_{-2}^3 
		\sqrt{16 - x^2 +  x^2 } \ dx
	\\&=
		2 \pi \int_{-2}^3 4 \ dx
	\\&=
		2 \pi (4x) \Big|_{-2}^3
	\\&=
		2 \pi (20)
	\\&=
		40 \pi
\end{align*}$$

![[Pasted image 20220304234743.png]]
$$\begin{align*}
	y' &= \frac{x^3}{2} - \frac 1 {2x^3} \\
	\\
	2 \pi \int_1^2 x
	\sqrt{1 + (\tfrac{x^3}{2} - \tfrac 1 {2x^3})^2}
	\ dx
	&=
		2 \pi \int_1^2 x
		\sqrt{1 + \tfrac{x^6}{4} + \tfrac 1 {4x^6} - \tfrac 1 2}
		\ dx \\
	\\&=
		2 \pi \int_1^2 x
		(\tfrac{x^3}{2} + \tfrac 1 {2x^3})
		\ dx \\
	\\&=
		2 \pi \int_1^2 
		\tfrac{x^4}{2} + \tfrac 1 {2x^2}
		\ dx \\
	\\&=
		2 \pi (\tfrac{x^5}{10} - \tfrac 1 {2x}) \Big|_1^2
	\\&=
		2 \pi (\tfrac{59}{20} - (- \tfrac 2 5)) \\
	\\&=
		\tfrac{67}{10} \pi
\end{align*}$$
