# A7 
*1)*
![[Pasted image 20220314140039.png]]
$$\begin{align*}
	\frac{dT}{dt}
	&=
		-k(T-9) \\
	\int T-9 \ dT
	&=
		-k \int \ dt \\
	\ln|T-9|
	&=
		-kt + c \\
	T-9
	&=
		e^{-kt+c} \\
	T
	&=
		Ce^{-kt} + 9 \\
	\\
	37 &= Ce^{-k0} + 9\\
	C &= 28 \\
	\\
	34 &= 28e^{-km} + 9 \\
	25 &= 28e^{-km} \\
	\frac{25}{28} &= e^{-km} \\
	\\
	16 &= 28e^{-k(m+3)} + 9 \\
	7 &= 28e^{-km-3k} \\
	\frac{1}{4} e^{3k} &= e^{-km} \\
	\\
	\frac{1}{4} e^{3k} &= \frac{25}{28} \\
	e^{3k} &= \frac{25}{7} \\
	k &= \frac{\ln(25/7)}{3} \\
	\\
	\frac{25}{28} &= e^{-\frac{\ln(25/7)}{3}m} \\
	\ln \frac{25}{28} &= -\frac{\ln(25/7)}{3}m \\
	m &= -\frac{\ln \frac{25}{28}}{\frac{\ln(25/7)}{3}} \\
\end{align*}$$

*2)*
![[Pasted image 20220314150246.png]]
$$\begin{align*}
	y(1) = 8 \Rightarrow
	y'(1) + 6(8) &= 0 \\
	y'(1) &= -48 \\
\end{align*}$$

$$\begin{align*}
	x^5y' + 6x^4y &= \frac{\ln x} x \\
	y' + 6x^{-1}y &= x^{-6} \ln x \\
	\frac d {dx} (x^6y) &= \ln x \\
	x^6y &= \int \ln x \ dx \\
	x^6y &= x \ln x - x + c \\
	y &= x^{-5} \ln x - x^{-5} + cx^{-6} \\
	y(1) = 8 \Rightarrow
	8 &= 1^{-5} \ln 1 - 1^{-5} + c(1)^{-6} \\
	8 &= - 1 + c \\
	9 &= c \\
	\\
	y(e) &= e^{-5} \ln e - e^{-5} + 9e^{-6} \\
	&= 9e^{-6}
\end{align*}$$

*3)*
![[Pasted image 20220314152032.png]]
$$\begin{align*}
	m_t' &= 3 - 0.15 m_t \\
	m_t' &= 0.15(20 - m_t) \\
	\ln|m_t-20| &= -0.15x + c \\
	m_t-20 &= ce^{-0.15x} \\
	m_t &= ce^{-0.15x} + 20 \\
	100 &= ce^{-0.15(0)} + 20 \\
	c &= 80 \\
	m_t &= 80e^{-0.15x} + 20 \\
	m_4 &= 80e^{-6/10} + 20
\end{align*}$$

*4)*
![[Pasted image 20220314152838.png]]
$$\begin{align*}
	x^2 - 1 &= t \\
	y^2 + 1 &= t \\
	\\
	x^2 - y^2 &= 2
\end{align*}$$

*6)*
![[Pasted image 20220314153318.png]]
$$\begin{align*}
	9 &= 2t^4 + 6t^2 + 1 \\
	0 &= t^4 + 3t^2 - 4 \\
	0 &= (t^2+4)(t^2-1) \\
	t &= \pm 1 \\
	\\
	0 &= 2t^3 - 2t \\
	0 &= 2t(t-1)(t+1) \\
	t &= 0, \pm 1 \\
	\\
	x' &= 8t^3 + 12t \\
	x' &= 4t(2t^2 + 3) \\
	\\
	y' &= 6t^2 - 2 \\
	y' &= 2(3t^2 - 2) \\
	\\
	y'(-1)/x'(-1) &= 4/-20 = -1/5 \\
	y'(1)/x'(1) &= 3/20 = 1/5 \\
\end{align*}$$