# 10.2
![[Pasted image 20220315134944.png]]

![[Pasted image 20220315135040.png]]
*a)*
$$\begin{align*}
	x &= \sin t \\
	\frac 1 2 &= \sin t \\
	t &= \frac \pi 6, \frac{5 \pi} 6 \\
	\\
	y &= \cos^2 t \\
	\frac 3 4 &= \cos^2 t \\
	\pm \frac{\sqrt 3} 2 &= \cos t \\
	t &= \frac \pi 6, \frac{5 \pi} 6 \\
	\\
	x' &= \cos t \\
	y' &= -2 \cos t \sin t \\
	\frac{dy}{dx}(t) &= \frac{-2 \cos t \sin t}{\cos t} \\
	&= -2 \sin t \\
	\\
	y - \frac 3 4 
	&= 
		\frac{dy}{dx}(\frac \pi 6)(x - \frac 1 2) \\
	y &= -x + \frac 1 2 + \frac 3 4 \\
	&= -x + \frac 5 4 \\
	\\
	y - \frac 3 4 
	&= 
		\frac{dy}{dx}(\frac{5 \pi} 6)(x - \frac 1 2) \\
	y &= -x + \frac 1 2 + \frac 3 4 \\
	&= -x + \frac 5 4
\end{align*}$$

*b)*
$$\begin{align*}
	x^2 &= \sin^2 t \\
	x^2 + y &= \sin^2 t + \cos^2 t \\
	x^2 + y &= 1 \\
	y &= -x^2 + 1 \\
	y' &= -2x \\
	y' -  \frac 3 4 &= y'(\frac 1 2)(x - \frac 1 2) \\
	y' &= -x + \frac 1 2 + \frac 3 4 \\
	y' &= -x + \frac 5 4
\end{align*}$$

![[Pasted image 20220315142638.png]]
$$\begin{align*}
	x' &= 2t \\
	y' &= 2t + 1 \\
	y'' &= 2 \\
	\\
	\frac{dy}{dx} &= \frac{dy/dt}{dx/dt} \\
	&= \frac{2t+1}{2t} \\
	&= 1 + \frac 1 {2t} \\
	\\
	\frac{d}{dx} \frac{dy}{dx}
	&=
		\frac d {dt} (1 + \frac 1 {2t}) / (2t) \\
	&=
		-\frac 1 {2t^2(2t)} \\
	&=
		-\frac 1 {4t^3}
\end{align*}$$

$$\begin{align*}
	-\frac{1}{4t^3} > 0 \\
	t^{-3} < 0 \\
	t < 0
\end{align*}$$

Thus $t$ must be $<0$.

![[Pasted image 20220315143734.png]]
$$\begin{align*}
	x' &= -\sin \theta \\
	y' &= -3 \sin 3 \theta \\
	\frac{dy}{dx}
	&=
		\frac{-3 \sin 3 \theta}{- \sin \theta} \\
	&=
		\frac{3 \sin 3 \theta}{\sin \theta} \\
	0 &=
		\frac{3 \sin 3 \theta}{\sin \theta} \\
	\sin 3 \theta &= 0 \\
	3\theta &= 0, \pi, 2\pi, 3\pi \\
	\theta &= 0, \frac \pi 3, \frac{2\pi}{3}, \pi,  \theta \neq 0, \pi
\end{align*}$$

So $\theta = \frac \pi 3, \frac{2\pi}{3}$ to make the curve horizontal.

$$\begin{align*}
	\lim_{x\to0} \frac{3 \sin 3 \theta}{\sin \theta}
	&=
		\lim_{x\to0} \frac{9 \cos 3 \theta}{\cos \theta}
	\\&=
		9
\end{align*}$$

Similar could be seen with $x \to \pi$, thus there's no vertical tangent.

![[Pasted image 20220315145554.png]]
$$\begin{align*}
	0 &= 2t - t^2 \\
	0 &= t(2-t) \\
	t &= 0, 2 \\
	x(0) &= 1, \\
	x(2) &= 9 \\
	\Rightarrow& (1, 0), (9, 0) \\
	\\
	\int_0^2 (2t-t^2)(3t^2) \ dt
	&=
		\int_0^2 -3t^4 + 6t^3 \ dt \\
	&=
		-\frac 3 5 t^5 + \frac 3 2 t^4 \Big|_0^2 \\
	&=
		\frac{24}{5}
\end{align*}$$

![[Pasted image 20220315151230.png]]
$$\begin{align*}
	\int_0^3 \sqrt{
		(\frac 2 3 t^3)^2 + (t^2-2)^2
	} \ dt
	&=
		\int_0^3 \sqrt{
			(2t^2)^2 + (2t)^2
		} \ dt
	\\&=
		\int_0^3 \sqrt{
			4t^4 + 4t^2
		} \ dt
	\\&=
		\int_0^3 2t\sqrt{
			t^2 + 1
		} \ dt
	\\&=
		\frac 2 3 (t^2+1)^{3/2} \Big|_0^3
	\\&=
		\frac 2 3(10)^{3/2} - \frac 2 3
\end{align*}$$

![[Pasted image 20220315152008.png]]
$$\begin{align*}
	&\int_0^1 \sqrt{
		(\sin t + t\cos t)^2 + (\cos t - t\sin t)^2
	} \ dt
	\\&=
		\int_0^1 \sqrt{
			\sin^2 t + 2t \sin t \cos t + t^2 \cos^2 t
			+
			\cos^2 t - 2t \sin t \cos t + t^2 \sin^2 t
		} \ dt
	\\&=
		\int_0^1 \sqrt{
			1 + t^2
		} \ dt
	\\&=
		\frac 1 2 x \sqrt{1 + x^2} 
		+
		\frac 1 2 \ln|x + \sqrt{1 + x^2}| \Big|_0^1
	\\&=
		\frac 1 2 \sqrt{2} 
		+
		\frac 1 2 \ln|1 + \sqrt{2}|
\end{align*}$$

![[Pasted image 20220315155344.png]]
$$\begin{align*}
	(2 \sin t \cos t)^2 + (-2 \cos t \sin t)^2
	&=
		2(\sin 2 t)^2 \\
	\\
	\int_0^{3 \pi} \sqrt{
		2 (\sin 2 t)^2
	} \ dt
	&= 
		\int_0^{3 \pi} \sqrt{
			2 
		} |\sin 2 t| \ dt
	\\&= 
		6 \sqrt 2 \int_0^{\pi / 2} 
		\sin 2 t \ dt
	\\&=
		3 \sqrt 2 \cos 2 t \Big|_0^{\pi/2}
	\\&=
		-3 \sqrt 2(-1 - 1)
	\\&=
		6 \sqrt 2
\end{align*}$$

![[Pasted image 20220315160427.png]]
$$\begin{align*}
	(3t^2)^2 + (2t)^2
	&=
		9t^4 + 4t^2 \\
	&=
		t^2(9t^2 + 4) \\
	\\
	2 \pi \int_0^1 t^2 \sqrt{
		9t^4 + 4t^2
	} \ dt
	&=
		2 \pi \int_0^1 t^2 \sqrt{
			t^2(9t^2 + 4)
		} \ dt
\end{align*}$$

Let $u = 9t^2 + 4 \implies du = 18t \implies \frac 1 {18} du = t \ dt$
$u = 9t^2 + 4 \implies t^2 = \frac{u-4}{9}$

$$\begin{align*}
	2 \pi \int_{4}^{13}
	\left( \frac{u - 4}{9} \right) \sqrt u \frac 1 {18} \ du
	&=
		\frac 1 {81} \pi \int_4^{13}
		u^{3/2} - 4u^{1/2} \ du
	\\&=
		\frac 1 {81} \pi (
			\frac{2}{5} u^{5/2}
			-
			\frac 8 3 u^{3/2}
		) \Big|^{13}_4
	\\&=
		\frac 1 {81} \pi (
			\frac{2}{5} 13^{5/2}
			-
			\frac 8 3 13^{3/2}
			-\frac{2}{5} 4^{5/2}
			+
			\frac 8 3 4^{3/2}
		)
\end{align*}$$