# 10.3
![[Pasted image 20220319133046.png]]

---
![[Pasted image 20220319140922.png]]
*a)*
$$\begin{align*}
	x &= 2 \cos(3 \pi / 2) \\
	&= 0 \\
	y &= 2 \cos(3 \pi / 2) \\
	&= -2 \\
	\Rightarrow
	(0, -2)
\end{align*}$$

*b)*
$$\begin{align*}
	x &= \sqrt 2 \cos(\pi/4) \\
	&= \sqrt 2 \frac{\sqrt 2}{2} \\
	&= 1
	\\
	y &= 1
	\Rightarrow
	(1,1)
\end{align*}$$

*c)*
$$\begin{align*}
	&(-\cos(-\pi / 6), -\sin(-\pi / 6)) \\
	&\Rightarrow
	(-\sqrt{3} / 2, 1/2)
\end{align*}$$

 ---
![[Pasted image 20220319140906.png]]

*i)*
$$\begin{align*}
	r^2 &= (-4)^2 + 4^2 \\
	r &= 4 \sqrt 2 \\
	\tan \theta &= \frac{-4} 4 \\
	\theta &= \frac{3 \pi}{4} \\
	&\Rightarrow (4 \sqrt 2, 3 \pi / 4)
\end{align*}$$

*ii)*
$$(-4 \sqrt 2, 7 \pi / 4)$$

*b)*
$$\begin{align*}
	r^2 &= (3)^2 + (3 \sqrt 3)^2 \\
	r &= 6 \\
	\tan \theta &= \frac{3 \sqrt 3} 3 \\
	\theta &= \frac{\pi}{3} \\
	&\Rightarrow
	(6, \pi/3)
\end{align*}$$

*ii)*
$$(-6, 4\pi/3)$$

---
![[Pasted image 20220319142426.png]]

![[Pasted image 20220319142411.png]]
$$\begin{align*}
	r^2 &= 5r \cos \theta \\
	x^2 + y^2 &= 5x \\
	x^2 - 5x + y^2 &= 0 \\
	(x - \tfrac 5 2)^2 + y^2 - \tfrac{25}{4} &= 0 \\
	(x - \tfrac 5 2)^2 + y^2 &= \tfrac{25}{4} \\
	(x - \tfrac 5 2)^2 + y^2 &= (\tfrac{5}{2})^2 \\
\end{align*}$$

Thus, it's a circle with radius $\tfrac 5 2$ centred at $(\tfrac 5 2, 0)$. Multiplying by $r$ is fine since equation can equal $0$ when $\theta = \tfrac \pi 2$.

---
![[Pasted image 20220319143725.png]]
$$\begin{align*}
	r^2(\cos^2 \theta - \sin^2 \theta) &= 1 \\
	x^2 - y^2 &= 1
\end{align*}$$

---
![[Pasted image 20220319144145.png]]

![[Pasted image 20220319144153.png]]
$$\begin{align*}
	(r \cos \theta)^2 + (r \sin \theta)^2 &= 7 \\
	r^2 &= 7 \\
	r^2 &= 7 \\
	r &= \sqrt 7
\end{align*}$$

$r = -\sqrt 7$ can be excluded since both equations produce the same curve.

---
![[Pasted image 20220319144405.png]]
$$\begin{align*}
	r \cos \theta &= -1 \\
	r &= - \sec \theta
\end{align*}$$
$\cos \theta = 0$ cannot happen since then the equation will become $0 = -1$ which is impossible.

---
![[Pasted image 20220319144556.png]]

$$\begin{align*}
	r^2 &= 4 r \sin \theta \\
	r &= 4 \sin \theta
\end{align*}$$

The 2 equations are equivalent since $\sin \theta$ can become 0 which will result in $r = 0$ anyways.

---
![[Pasted image 20220319145035.png]]
![[Pasted image 20220319145041.png]]
![[Pasted image 20220319145102.png]]

*a)* 
- Intersects the origin since $\cos(3 \tfrac \pi 6) = 0$
- Has max $r$ values at $\theta = 0, \tfrac \pi 3, \frac{2 \pi} 3, \pi$, or $(1, 0), (-1, \tfrac \pi 3), (1, \frac{2 \pi}{3}), (-1, \pi)$
Thus it's *II*

*b)* Since $r = \ln \theta$, it is an increasing function and since $1 \le \theta$, it must start at an angle. Thus it's *VI*.

*c)* 
- Intersects the origin when $\theta = \pi$.
-  As $\theta$ increases to $\pi$, the $r$ decreases. 
thus is must be *V*

*d)*
- As $\theta$ increases to $3\pi/2$, $r$ decreases. 
Must be *IX*

*e)*
- No origin intersection
- As $\theta$ increases to $\frac{3\pi}{2}$, $r$ approaches infinity.
Must be $VII$

*f)*
$$r \cos \theta = 1 \Rightarrow x = 1$$
So it's *VIII*

*g)*
- 8/2 = 4 revolutions
- *III*

*h)*
- *IV* Since 3 leafed rose but does not intersect the origin

*i)*
- $I$.

