# 11.10
![[Pasted image 20220217000746.png]]
![[Pasted image 20220217000821.png]]

$$\begin{align*}
	f'(x) &= 2(1-x)^{-3} \\
	f''(x) &= 2\cdot 3(1-x)^{-4} \\
	So \\
	f^{(n)}(x) &= (n+1)!(1-x)^{-n-2} \\
	\\
	f(x) &= \sum_{n = 0}^\infty \frac{(n+1)!(1-0)^{-n-2}}{n!} x^n \\
	&= \sum_{n = 0}^\infty (n+1) x^n \\
\end{align*}$$

And it is clear that $R=1$.

![[Pasted image 20220217002451.png]]

$$\begin{align*}
	\sin x &= \sum_{n=0}^\infty (-1)^n \frac{x^{2n+1}}{(2n+1)!} \\
	\frac d {dx} \sin x &= \frac d {dx} \sum_{n=0}^\infty (-1)^n \frac{x^{2n+1}}{(2n+1)!} \\
	\cos x &= \sum_{n=0}^\infty (-1)^n \frac{(2n+1)x^{2n}}{(2n+1)!} \\
	\cos x &= \sum_{n=0}^\infty (-1)^n \frac{x^{2n}}{(2n)!} \\
\end{align*}$$

$$\begin{align*}
	\lim_{n\to\infty} \left| 
		(-1)^n 
		\frac {x^{2(n+1)}} {(2(n+1))!}
		\cdot
		\frac {(2n)!} {x^{2n}}
	\right|
	\\
	\lim_{n\to\infty} \left| 
		\frac {x^{2n+2}} {(2n+2)!}
		\cdot
		\frac {(2n)!} {x^{2n}}
	\right|
	\\
	\lim_{n\to\infty} \left| 
		\frac {x^{2}} {(2n+2)(2n+1)}
	\right| &< 1
	\\
	0 &< 1
\end{align*}$$

$\therefore$ the radius of convergence is $(-\infty, \infty)$

![[Pasted image 20220217003432.png]]
The power series is the function. It has a radius of convergence of $\infty$.

![[Pasted image 20220217003929.png]]
$$\begin{align*}
	f'(x) &= 2e^{2x} \\
	f^{(n)}(x) &= 2^ne^{2x} \\
	f(x) &= \sum_{n=0}^\infty \frac{2^n e^{2(3)}}{n!} (x-3)^n \\
	f(x) &= \sum_{n=0}^\infty \frac{2^n e^6}{n!} (x-3)^n \\
	f(x) &= e^6 \sum_{n=0}^\infty \frac{2^n}{n!} (x-3)^n \\
\end{align*}$$

$$\begin{align*}
	\lim_{n\to\infty} \left| \frac{2^{n+1}}{(n+1)!} (x-3)^{n+1} \cdot \frac{n!}{2^n (x-3)^n} \right|
	&=
		\lim_{n\to\infty} \left| \frac{2}{n+1} (x-3) \right| \\
	&=
		0 < 1
\end{align*}$$

$\therefore$ the radius of convergence is $\infty$.

![[Pasted image 20220217005408.png]]
$$\begin{align*}
	(1-x)^\frac 1 4 &= \sum_{n=0}^\infty \frac{\frac 1 4\cdots(\frac 1 4 - n + 1)}{n!} (-x)^n \\
	&=
		1 + \frac 1 4 (-x) + \frac 1 4 (-\frac 3 4)(-x)^2 + \frac 1 4 (-\frac 3 4 )(-\frac 7 4)(-x)^3 + \cdots \\
	&= 1 - \frac 1 4 x -\sum_{n=2}^\infty \frac {3 \cdots (4n-5)} {4^{n} n!}x^{n}
		
\end{align*}$$

Radius of convergence:
$$\begin{align*}
	&\lim_{n\to\infty} \left|
		\frac {3 \cdots (4n-1)} {4^{n+1} (n+1)!}x^{n+1}
		\cdot
		\frac {4^{n} n!} {3 \cdots (4n-5)x^{n}}
	\right| \\
	&= 
	\lim_{n\to\infty} \left|
		\frac {4n-1} {4 (n+1)}x
	\right| \\
	&= 
		|x| < 1
\end{align*}$$

$\therefore$ the radius of convergence is length 1.

![[Pasted image 20220217095627.png]]
$$\begin{align*}
	f'(x) &= -xe^{-x}+e^{-x} \\
	f''(x) &= xe^{-x}-2e^{-x} \\
	f^{(n)}(x) &= (-1)^n xe^{-x} + (-1)^{n+1} ne^{-x} \\
	f(x) &= \sum_{n=0}^\infty
		\frac{(-1)^n (0)e^{-0}+(-1)^{n+1}ne^{-0}}{n!} x^n \\
	&= \sum_{n=0}^\infty
		\frac{(-1)^{n+1} n}{n!} x^n \\
	&= \sum_{n=1}^\infty
		\frac{(-1)^{n+1}}{(n-1)!} x^n \\
\end{align*}$$

$$\begin{align*}
	&\lim_{n\to\infty} \left|
		\frac{(-1)^{n+2}}{n!} x^{n+1}
		\cdot
		\frac{(n-1)!}{(-1)^{n+1} x^n}
	\right| \\
	&=
	\lim_{n\to\infty} \left|
		\frac{1}{n} x
	\right| \\
	&=
		0
\end{align*}$$

So radius of convergence is $\infty$, and interval of convergence is also $\infty$.

$$\begin{align*}
	\text{Let } f(x) &= T_n(x)+R_n(x) \\
	\text{Then} \\
	|x| &\leq \infty \\
	\text{All the time, so any d>0 works.} \\
	\text{So let d be any positive real number greater than x. Then} \\
	|f^{(n)}(x)| = (-1)^nxe^{-x}+(-1)^{n+1} n e^{-x} \leq de^{d}+ne^{d}
\end{align*}$$
Thus we have found an $M$ such taht
$$|R_n(x)| = \frac{M}{(n+1)!}|x^{n+1}|$$
which approaches 0 as $n \to \infty$.

So $f(x)$ is equal to its taylor series.

![[Pasted image 20220217143140.png]]
$$\begin{align*}
	&= \int \sqrt{1+x^3}\ dx \\
	&= \int 
		\sum_{n=0}^\infty
			\binom{\frac 1 2}{n}(x^3)^n
	\ dx \\
	&= 
		\sum_{n=0}^\infty \binom{\frac 1 2}{n} \frac{
			x^{3n+1}
		} {
			3n+1
		}
	\\
\end{align*}$$

$$\begin{align*}
	&\lim_{n\to\infty}
		\binom{\frac 1 2}{n+1} \frac{
			x^{3n+4}
		} {
			3n+4
		}
		\cdot
		\frac{
			 3n+1
		} {
			\binom{\frac 1 2}{n}x^{3n+1}
		} \\
	&= \lim_{n\to\infty} \left|
		\frac{
			(\frac 1 2 + n)(3n+1)
		} {
			(n+1)(3n+4)
		}x^{3} \right|
		\\
	&= |x^3|
\end{align*}$$

So radius of convergence is 1.

![[Pasted image 20220217151517.png]]
$$\begin{align*}
	&\int \frac{
		\sum_{n=0}^\infty (-1)^n \frac{
			x^{2n}
		}{
			(2n)!
		} 
	}{x}
	- \frac 1 x
	\ dx \\
	&=
		\int \frac{
			x\sum_{n=0}^\infty (-1)^n \frac{
				x^{2n-1}
			}{
				(2n)!
			} 
		}{x}
		- \frac 1 x
		\ dx \\
	&=
		\int
			\sum_{n=1}^\infty (-1)^n \frac{
				x^{2n-1}
			}{
				(2n)!
			} 
		\ dx \\
	&=
			\sum_{n=1}^\infty (-1)^n \frac{
				x^{2n}
			}{
				(2n)!(2n)
			} + c
\end{align*}$$

![[Pasted image 20220217153053.png]]
$$\begin{align*}
	e^{-x^4}
\end{align*}$$