# 7.4 - Comparison Tests
![[Pasted image 20220203095916.png]]

 ![[Pasted image 20220203100006.png]]
 $\because \sum_{n=1}^\infty \frac{1}{n^3+8}$ is positive for all $n \geq 1$, we can compare to another series:
$$\begin{align*} 
	\sum_{n=1}^\infty \frac{1}{n^3+8}
		&\leq \sum_{n=1}^\infty \frac{1}{n^3}
\end{align*}$$
$\because \sum_{n=1}^\infty \frac{1}{n^3}$  is a p-series with $p = 3 \geq 1$ and $a_n \leq b_n$, we have that the series converges.

![[Pasted image 20220203101039.png]]

$\because \sum_{n=1}^\infty \frac{n+1}{n \sqrt{n}}$ is positive for all $n \geq 1$, we can compare to another positive series:
$$\begin{align*}
	\sum_{n=1}^\infty \frac{n+1}{n \sqrt{n}}
		&\geq \sum_{n=1}^\infty \frac{n}{n \sqrt{n}} \\
		&\geq \sum_{n=1}^\infty \frac{1}{\sqrt{n}} \\
\end{align*}$$
$\because \sum_{n=1}^\infty \frac{1}{\sqrt{n}}$ is a p-series with $p=\frac{1}{2} \leq 1$ and $a_n \geq b_n$, the series diverges

![[Pasted image 20220203103444.png]]

$\because (\forall n \in \mathbb{R})(\sum_{n=1}^\infty \frac{9^n}{3+10^n} > 0)$, we can compare to another series.
$$\begin{align*}
	\sum_{n=1}^\infty \frac{9^n}{3+10^n}
		&\leq \sum_{n=1}^\infty \left(\frac{9}{10}\right)^n
\end{align*}$$
$\because \sum_{n=1}^\infty \left(\frac{9}{10}\right)^n>0$ is a geometric series with with $|r|<1$ and $a_n\geq b_n$, the series converges.

![[Pasted image 20220203104315.png]]

Notice: $(\forall n \in \mathbb{R})(n>0 \to \frac{1}{\ln(n)}>0)$, so we can use the direct comparison test.
$$\begin{align*}
	n &\leq \ln(n) \\
	\frac{1}{n} &\leq \frac{1}{\ln(n)} \\
	\sum_{n=2}^\infty \frac{1}{n} &\leq \sum_{n=2}^\infty \frac{1}{\ln(n)}
\end{align*}$$
$\because \sum_{n=2}^\infty \frac{1}{n}$ is the harmonic series, it diverges. Since $a_n \leq b_n$, then the given series also diverges.

![[Pasted image 20220203105607.png]]

Notice: $(\forall n \in \mathbb{Z})(n \geq 1 \to \frac{1+\cos(n)}{e^n}>0)$, so we can use the direct comparison test.
$$\begin{align*}
	\sum_{n=1}^\infty \frac{1+\cos(n)}{e^n}
		&\leq \sum_{n=1}^\infty \frac{2}{e^n} \\
		&\leq \sum_{n=2}^\infty \frac{2}{e^n}
			+\frac{2}{e}
\end{align*}$$
$\because$ the compared series is greater than 0 for all terms and is a p-series with $p>1$, we have that the original series is convergent.

![[Pasted image 20220203110828.png]]
$$\begin{align*}
	\sum_{n=1}^\infty \frac{4^{n+1}}{3^n-2}
		&\geq 4 \cdot \sum_{n=1}^\infty \frac{4^n}{3^n} \\
		&\geq \frac{16}{3} \cdot \sum_{n=1}^\infty \left(\frac{4}{3}\right)^{n-1}
\end{align*}$$
$\because$ both series have positive terms, can use the direct comparison test. The second series a geometric series with $|r|=\frac{4}{3}>1$ and all terms less than the og series so the og series is divergent.

![[Pasted image 20220203111401.png]]
$$\begin{align*}
	\lim_{n \to \infty} \frac{\frac{\sqrt{1+n}}{2+n}}{\frac{\sqrt{n}}{2+n}}
		&= \lim_{n \to \infty} \frac{\sqrt{1+n}}{\sqrt{n}} \\
		&= 1
\end{align*}$$
$\because$ Both series in the limit have positive terms, and $c=1>0$, then both series converge or diverge.
$$\begin{align*}
	\lim_{n\to\infty} \frac{\frac{\sqrt{n}}{2+n}}{\frac{\sqrt{n}}{n}} = 1
\end{align*}$$
$\because$ both series in the limit have positive terms, and $c=1>0$, then both series converge or diverge.
$$
	\sum_{n=1}^\infty \frac{\sqrt{n}}{n}
		= \sum_{n=1}^\infty \frac{1}{\sqrt{n}}
$$
$\because$ the series is a p-series with $p=\frac{1}{2}>1$, we have that it diverges. Therefore, the og series diverges by transitivity law.

![[Pasted image 20220203113358.png]]
$$\begin{align*}
	\lim_{n\to\infty} \frac{\frac{e^n+1}{ne^n+1}}{\frac{e^n}{ne^n}}
	&= \lim_{n\to\infty}
		\left(\frac{e^n+1}{e^n}\right)
		\left(\frac{ne^n}{ne^n+1}\right) \\
	&= \lim_{n\to\infty} \left(\frac{e^n+1}{e^n}\right)
		\lim_{n\to\infty} \left(\frac{ne^n}{ne^n+1}\right) \\
	&= 1
\end{align*}$$
$\because$ both series in the limit have positive terms, and $c=1>0$, then both series converge or diverge.
$$\begin{align*}
	\sum_{n=1}^\infty \frac{e^n}{ne^n}
		&= \sum_{n=1}^\infty \frac{1}{n}
\end{align*}$$
$\because$ the series is the harmonic series, the sum of the series diverges.
$\therefore$ the original sum also diverges.