# 11.6

![[Pasted image 20220207154314.png]]
![[Pasted image 20220207154526.png]]
$$\begin{align*}
	\sum_{n=1}^\infty (-1)^{n-1} \frac{3^n}{2^nn^3}
		&\Rightarrow 
			\lim_{n\to\infty} \left|\frac{
				(-1)^{n+1-1}\frac{3^{n+1}}{2^{n+1}(n+1)^3}
			}{
				(-1)^{n-1}\frac{3^n}{2^nn^3}
			}\right| \\
		&=
			\lim_{n\to\infty} \left|
				\frac{3 \cdot 3^n}{2 \cdot 2^n(n+1)^3}
				\cdot
				\frac{2^nn^3}{3^n}
			\right| \\
		&=
			\lim_{n\to\infty} \left|
				\frac{3}{2 \cdot (n+1)^3}
				\cdot
				n^3
			\right| \\
		&=
			\lim_{n\to\infty} \left|
				\frac{3}{n^3 \cdot 2 \cdot (1+\frac{1}{n^3})^3}
				\cdot
				n^3
			\right| \\
		&=
			\lim_{n\to\infty} \left|
				\frac{3}{2 \cdot (1+\frac{1}{n^3})^3}
			\right| \\
		&= \frac{3}{2}
\end{align*}$$
$\because L>1$, the series is divergent by the Ratio Test.

![[Pasted image 20220207163557.png]]
$$\begin{align*}
	\sum_{n=1}^\infty \frac{2 \cdot 4 \cdot 6 \cdot \cdots \cdot (2n)}{n!}
		&= \sum_{n=1}^\infty \frac{2^nn!}{n!} \\
		&= \sum_{n=1}^\infty 2^n
\end{align*}$$
But the series is a geometric series with $r=2>1$ so the series is divergent.

![[Pasted image 20220207164002.png]]
$$\begin{align*}
	\sum_{n=1}^\infty \left(\frac{
		n^2+1
	}{
		2n^2+1
	}\right)^n
	&\Rightarrow
		\lim_{n\to\infty} \sqrt[n]{\left|\left(\frac{
			n^2+1
		}{
			2n^2+1
		}\right)^n\right|} \\
	&=
		\lim_{n\to\infty} \left|\frac{
			1+\frac{1}{n^2}
		}{
			2+\frac{1}{n^2}
		}\right| 
	\\&= \frac 1 2
\end{align*}$$
$\because L<1$, the series is absolutely divergent by the root test.

![[Pasted image 20220207165124.png]]
$$\begin{align*}
	\sum_{n=1}^\infty \left(
		1+\frac 1 n
	\right)^{n^2}
	&\Rightarrow
		\lim_{n\to\infty} \sqrt[n]{\left|
			1+\frac 1 n
		\right|^{n^2}}
	\\&=
		\lim_{n\to\infty} \left|
			1+\frac 1 n
		\right|^n
	\\&= e
\end{align*}$$
$\because L>1$, the series is divergent.

![[Pasted image 20220207165756.png]]
$(\forall n \geq 2)(\frac{\ln n}{n} \geq \frac{\ln(n+1)}{n+1})$.
$$\begin{align*}
	\Rightarrow
	\lim_{n\to\infty} \frac{
		(-1)^n \ln n
	} n
	&\Rightarrow
		\lim_{n\to\infty} \left|\frac{
			(-1)^n \ln n
		} n \right|
	\\&=
		\lim_{n\to\infty} \left|\frac{
			\frac 1 n
		} 1 \right|
	\\&= 0
\end{align*}$$
$\because L=0$, the series is absolutely convergent by the alternating series test.

![[Pasted image 20220207170634.png]]
$$\begin{align*}
	\Rightarrow \lim_{n\to\infty} \left|\frac{
		\frac{5n+1}{4n+3} a_n
	}{
		\frac{5(n-1)+1}{4(n-1)+3} a_{n-1}
	}\right|
	&=
		\lim_{n\to\infty} \left|\frac{
			\frac{5n+1}{4n+3} 
			\cdot
			\frac{5(n-1)+1}{4(n-1)+3} a_{n-1}
		}{
			\frac{5(n-1)+1}{4(n-1)+3} a_{n-1}
		}\right|
	\\&=
		\lim_{n\to\infty} \left|
			\frac{5n+1}{4n+3} 
		\right|
	\\&= \frac 5 4
\end{align*}$$

$\because L>1$, by the ratio test, the series is divergent.