# 11.8
![[Pasted image 20220210142522.png]]
![[Pasted image 20220210142534.png]]
$$\begin{align*}
	\lim_{n\to\infty} \left| \frac{
		\frac{1}{n+1} x^{n+1}
	} {
		\frac 1 n x^n
	} \right|
	&= 
		\lim_{n\to\infty} \left| \frac{
			1
		} {
			1 + \frac 1 n
		} x \right|
	\\&=
		|x|<1
\end{align*}$$
$\therefore$ the radius of convergence is 1.
When $|x|=1$, $x=\pm 1$. When $x=1$, the series is the harmonic series and thus diverges. When $x=-1$, the series is the alternating harmonic series which diverges by the alternating series test.
$\therefore$ the interval of convergence $x \in [-1,1)$.

![[Pasted image 20220210145307.png]]
$$\begin{align*}
	\lim_{n\to\infty} \left| \frac{
		\frac{x^{n+1}}{2(n+1)-1}
	} {
		\frac{x^n}{2n-1}
	} \right|
	&=
		\lim_{n\to\infty} \left| x \frac{
			2n-1
		} {
			2n+1
		} \right|
	\\&= |x|
\end{align*}$$
$\therefore$ the radius of convergence is 1.
When $|x|=1$, $x=\pm 1$.
##### Case 1: $x=1$
$$\begin{align*}
	\lim_{n\to\infty} \frac{
		\frac 1 n
	}{
		\frac{1}{2n-1}
	}
	&=
		\lim_{n\to\infty} 2 - \frac 1 n
	\\&= 2 > 0
\end{align*}$$
Then, since $\frac 1 n$ is the harmonic series which diverges, $\frac{1}{2n-1}$ also diverges by the limit comparison test.
##### Case 2: $x=-1$
The series is positive, decreasing, and the limit approaches 0. Then, by the alternating series test, the series is converging.
$\therefore$ the interval of convergence is $x \in [-1, 1)$

![[Pasted image 20220210151417.png]]
$$\begin{align*}
	\lim_{n\to\infty} \left| (-1)^n \frac{
		\frac{4^{n+1}}{\sqrt{n+1}} x^{n+1}
	}{
		\frac{4^n}{\sqrt n}
	} \right|
	&=
		\lim_{n\to\infty} \left| 4x \sqrt{\frac{
			n
		}{
			n+1
		}}\right|
	\\&= 4|x| < 1
	\\&= |x|<\frac 1 4
\end{align*}$$
$\therefore$ the radius of convergence is $\frac 1 4$

When $|x|=\frac 1 4$, $x = \pm \frac 1 4$

##### Case 1: $x = \frac 1 4$
Then the series is an alternating series with decreasing terms and a limit that approaches 0. Then by the alternating series test, the series is convergent.

##### Case 2: $x = -\frac 1 4$
Then the series is a p-series with $p = \frac 1 2 < 1$, so therefore it diverges.

$\therefore$ the interval of convergence is $x \in (-\frac 1 4, \frac 1 4]$

![[Pasted image 20220210153446.png]]
$$\begin{align*}
	\lim_{n\to\infty} \left| \frac{
		\frac{(x-2)^{n+1}}{(n+1)^2+1}
	}{
		\frac{(x-2)^n}{n^2+1}
	} \right|
	&=
		\lim_{n\to\infty} \left| (x-2) \frac{
			n^2+1
		}{(n+1)^2+1}\right|
	\\&=
		|x-2|
\end{align*}$$
$\therefore$ the radius of convergence is 1

When $|x-2|=1, x=2 \pm 1$

##### Case 1: $x=3$
Then the series is convergent by comparison theorem with $\frac 1 {n^2}$.

##### Case 2: $x = 1$
Then the series is convergent because terms are decreasing and the limit approaches 0 and it's alternating so it's convergent by the alternating series test.

$\therefore$ The interval of convergence is $x \in [1, 3]$

![[Pasted image 20220210154504.png]]
$$\begin{align*}
	\lim_{n\to\infty} \left| \frac{
		\frac{(x+2)^{n+1}}{2^{n+1} \ln(n+1)}
	}{
		\frac{(x+2)^n}{2^n \ln n}
	} \right|
	&=
		\lim_{n\to\infty} \left| \frac{(x+2)}{2} \frac{
			\ln n
		}{
			\ln(n+1)
		} \right|
	\\&=
		\left| \frac{(x+2)}{2} \right| < 1
	\\&= |x+2| < 2
\end{align*}$$
$\therefore$ the radius of convergence is 2

when $|x+2|=2, x = -2 \pm 2$

##### Case 1: $x = 0$
$$\begin{align*}
	\frac{1}{\ln n} > \frac 1 n
\end{align*}$$
But $\frac 1 n$ is the harmonic series so it diverges, so by comparison test, $\frac 1 {\ln n}$ also diverges.

##### Case 2: $x=-4$
The series is an alternating series with decreasing terms and and a limit that approaches 0, so it is convergent by the alternating series test.

$\therefore$ the interval of convergence is $x \in [-4, 0)$

![[Pasted image 20220210160233.png]]
$$\begin{align*}
	\lim_{n\to\infty} \left| \frac{
		(n+1)!(2x-1)^{n+1}
	}{
		n!(2x-1)^n
	} \right|
	&=
		\lim_{n\to\infty} |(n+1)(2x-1)|
\end{align*}$$
##### Case 1: $x \neq \frac 1 2$
$$\lim_{n\to\infty} |(n+1)(2x-1)| = \infty$$
So the series diverges.

##### Case 2: $x = \frac 1 2$
$$\lim_{n\to\infty} |(n+1)(2 \left( \frac 1 2 \right)-1)| = 0$$
So the series converges.

$\therefore$ the radius of convergence is 0 and the interval of convergence is $x \in \{\frac 1 2\}$

![[Pasted image 20220210161445.png]]
$$\begin{align*}
	&= \sum \frac{x^n 2^n n!}{(2n)!}
	\\&\Rightarrow
		\lim_{n\to\infty} \left| \frac{
			\frac{x^{n+1} 2^{n+1} (n+1)!}{(2(n+1))!}
		}{
			\frac{x^n 2^n n!}{(2n)!}
		} \right|
	\\&=
		\lim_{n\to\infty} \left| 2x(n+1) \frac{
			(2n)!
		}{
			(2n+2)!
		} \right|
	\\&=
		\lim_{n\to\infty} \left| 2x(n+1) \frac{
			1
		}{
			(2n+1)(2n+2)
		} \right|
	\\&= 0
\end{align*}$$
$\therefore$ the radius of convergence is $\infty$ and the interval of convergence is $x \in (-\infty,\infty)$

![[Pasted image 20220210163854.png]]
$$\begin{align*}
	\lim_{n\to\infty} \left| \frac{
		c_{n+1}4^{n+1}
	}{
		c_n4^n
	} \right|
	&=
		\lim_{n\to\infty} \left| 4 \frac{
			c_{n+1}
		}{
			c_n
		} \right|
	\\1 &=
		4 \lim_{n\to\infty} \left| \frac{
			c_{n+1}
		}{
			c_n
		} \right|
	\\\frac 1 4 &= 
		\lim_{n\to\infty} \left| \frac{
			c_{n+1}
		}{
			c_n
		} \right|
\end{align*}$$
*a)*
$$\begin{align*}
	\lim_{n\to\infty} \left| \frac{
		c_{n+1}(-2)^{n+1}
	}{
		c_n(-2)^n
	} \right|
	&=
		\lim_{n\to\infty} \left| -2 \frac{
			c_{n+1}
		}{
			c_n
		} \right|
	\\&=
		2 \lim_{n\to\infty} \left| \frac{
			c_{n+1}
		}{
			c_n
		} \right|
	\\&= 2 \left(\frac 1 4 \right)
	\\&= \frac 1 2 < 1
\end{align*}$$
$\therefore$ the series is convergent by the ratio test.

*b)*
$$\begin{align*}
	\lim_{n\to\infty} \left| \frac{
		c_{n+1}(-4)^{n+1}
	}{
		c_n(-4)^n
	} \right|
	&=
		\lim_{n\to\infty} \left| -4 \frac{
			c_{n+1}
		}{
			c_n
		} \right|
	\\&=
		4 \lim_{n\to\infty} \left| \frac{
			c_{n+1}
		}{
			c_n
		} \right|
	\\&= 4 \left(\frac 1 4 \right)
	\\&= 1
\end{align*}$$
$\therefore$ no conclusion can be made.

![[Pasted image 20220210171457.png]]

*a)*
$$\begin{align*}
	\lim_{n\to\infty} \left| \frac{
		c_{n+1} x^{n+1}
	}{
		c_n x^n
	} \right|
	&=
		\lim_{n\to\infty} \left| x \frac{
			c_{n+1}
		}{
			c_n
		} \right|
	\\\text{if } x=-4 \Rightarrow 1 &>
		\lim_{n\to\infty} \left| -4 \frac{
			c_{n+1}
		}{
			c_n
		} \right|
	\\\frac{1}{4} &>
		\lim_{n\to\infty} \left| \frac{
			c_{n+1}
		}{
			c_n
		} \right|
	\\\text{if } x=6 \Rightarrow 1 &<
		\lim_{n\to\infty} \left| 6 \frac{
			c_{n+1}
		}{
			c_n
		} \right|
	\\\frac{1}{6} &<
		\lim_{n\to\infty} \left| \frac{
			c_{n+1}
		}{
			c_n
		} \right|
\end{align*}$$
Then,
$$
	\frac{1}{6} <
	\lim_{n\to\infty} \left| 
		\frac{ c_{n+1} }{ c_n }
	\right|
	< \frac{1}{4}
$$
*a)* Converges
*b)* 
$$\begin{align*}
	\\\text{if } x=8 \Rightarrow 
		&\lim_{n\to\infty} \left| 8 \frac{
			c_{n+1}
		}{
			c_n
		} \right|
		\\
		\frac 1 6 \cdot 8 <\
		&8\lim_{n\to\infty} \left| \frac{
			c_{n+1}
		}{
			c_n
		} \right|
		< \frac 1 4 \cdot 8
		\\
		1 < \frac 4 3 <\
		&8\lim_{n\to\infty} \left| \frac{
			c_{n+1}
		}{
			c_n
		} \right|
		< 2
\end{align*}$$
$\therefore$ diverges
*c)*
$$\begin{align*}
	\\\text{if } x=-3 \Rightarrow 
		&\lim_{n\to\infty} \left| (-3) \frac{
			c_{n+1}
		}{
			c_n
		} \right|
		\\
		\frac 1 6 \cdot 3 <\
		&3\lim_{n\to\infty} \left| \frac{
			c_{n+1}
		}{
			c_n
		} \right|
		< \frac 1 4 \cdot 3
		\\
		\frac 1 2 <\
		&3\lim_{n\to\infty} \left| \frac{
			c_{n+1}
		}{
			c_n
		} \right|
		< \frac 3 4 < 1
\end{align*}$$
$\therefore$ converges
*d)*
$$\begin{align*}
	\\\text{if } x=-9 \Rightarrow 
		&\lim_{n\to\infty} \left| (-9) \frac{
			c_{n+1}
		}{
			c_n
		} \right|
		\\
		\frac 1 6 \cdot 9 <\
		&9\lim_{n\to\infty} \left| \frac{
			c_{n+1}
		}{
			c_n
		} \right|
		< \frac 1 4 \cdot 9
		\\
		1 < \frac 3 2 <\
		&9\lim_{n\to\infty} \left| \frac{
			c_{n+1}
		}{
			c_n
		} \right|
		< \frac 9 4
\end{align*}$$
$\therefore$ diverges