# 11.9
![[Pasted image 20220213005941.png]]

![[Pasted image 20220213010003.png]]
$$\begin{align*}
	f(x) 
		&=
			\frac{2}{3-x}
		\\&=
			\frac{2}{3}\left(
				\frac{1}{1-\frac x 3}
			\right)
		\\&=
			\frac 2 3 \sum \left( \frac x 3 \right)^n
\end{align*}$$
So interval of convergence is $(-3, 3)$

![[Pasted image 20220213010728.png]]
$$\begin{align*}
	f(x)
		&= 
			\frac{x^2}{x^4+16}
		\\&=
			-\frac 1 {16} \frac{x^2}{-\frac{x^4}{16}-1}
		\\&=
			-\frac{x^2}{16} \sum \left( -\frac{x^4}{16} \right)^n
\end{align*}$$
So the interval of convergence is (-2, 2)

![[Pasted image 20220213095309.png]]
$$\begin{align*}
	f(x) 
		&=
			\frac{x-1}{x+2}
		\\&=
			\frac{x-1+3-3}{x+2}
		\\&=
			1-\frac{3}{x+2}
		\\&=
			1-\frac 3 2 \cdot \frac 1 {-\left( -\frac x 2 \right) + 1}
		\\&=
			1 - \frac 3 2 \sum \left( -\frac x 2 \right)^n
		\\&=
			1 - \sum_{n=0}^\infty 
			\frac{(-1)^n 3 x^n}{2^{n+1}}
		\\&=
			1-\frac 3 2 - \sum_{n=1}^\infty 
			\frac{(-1)^n 3 x^n}{2^{n+1}}
		\\&=
			-\frac 1 2 - \sum_{n=1}^\infty 
			\frac{(-1)^n 3 x^n}{2^{n+1}}
\end{align*}$$
$$\begin{align*}
	\left| -\frac x 2 \right|<1
	\\ -2<x<2
\end{align*}$$
#### Case 1: $x=-2$
$$\begin{align*}
		\\&=
			1 - \frac 3 2 \sum \left( -\frac {-2} 2 \right)^n
		\\&=
			1-\frac 3 2 \sum_{n=0}^\infty 1
		\\&=
			-\infty
\end{align*}$$
$\therefore$ the series is divergent for $x=-2$

#### Case 2: $x=2$
$$\begin{align*}
		&=
			1 - \frac 3 2 \sum \left( -\frac 2 2 \right)^n
		\\&=
			1 - \frac 3 2 \sum_{n=0}^\infty (-1)^n
\end{align*}$$
$\because$ the series fails the test for divergence, it is divergent.

![[Pasted image 20220213105847.png]]

*a)*
$$\begin{align*}
	\frac d {dx}\frac 1 {1+x} 
		&= \frac d {dx}\sum_{n=0}^\infty (-1)^n x^n
	\\ -\frac 1 {(1+x)^2} 
		&= \sum_{n=1}^\infty (-1)^n n x^{n-1}
	\\ \frac 1 {(1+x)^2} 
		&= -\sum_{n=1}^\infty (-1)^n n x^{n-1}
		\\&= -\sum_{n=0}^\infty (-1)^{n+1} (n+1) x^n
		\\&= \sum_{n=0}^\infty (-1)^n (n+1) x^n
\end{align*}$$
The radius of convergence is the same as the og radius of convergence, which is 1.

*b)*
$$\begin{align*}
	\frac d {dx} \frac 1 {(1+x)^2}
		&= \frac d {dx} \sum_{n=0}^\infty (-1)^n (n+1) x^n
	\\ \frac{-2}{(1+x)^3}
		&= \sum_{n=1}^\infty (-1)^n(n+1)nx^{n-1}
	\\ \frac{1}{(1+x)^3}
		&= 
			\frac{1}{2} \sum_{n=0}^\infty
			(-1)^n(n+1)(n+2)x^n
	\\ \frac{1}{(1+x)^3}
		&= 
			\frac{1}{2} \sum_{n=0}^\infty
			(-1)^n(n+1)(n+2)x^n
\end{align*}$$
$R=1$

*c)*
$$\begin{align*}
	x^2 \cdot \frac{1}{(1+x)^3}
		&= 
			x^2 \cdot \frac{1}{2} \sum_{n=0}^\infty
			(-1)^n(n+1)(n+2)x^n
	\\ \frac{x^2}{(1+x)^3}
		&= 
			\frac{1}{2} \sum_{n=0}^\infty
			(-1)^n(n+1)(n+2)x^{n+2}
	\\ \frac{x^2}{(1+x)^3}
		&= 
			\frac{1}{2} \sum_{n=2}^\infty
			(-1)^n(n-1)nx^n
\end{align*}$$
![[Pasted image 20220213122119.png]]
$$\begin{align*}
	\ln(5-x)
		&= 
			-\int \frac 1 {5-x}\ dx
		\\&=
			-\int \frac 1 {5(1 - \frac x 5)}\ dx
		\\&=
			-\int \sum_{n=0}^\infty \frac 1 5 5^{-n} x^n\ dx
		\\&=
			-\sum_{n=0}^\infty 5^{-n-1} \frac{x^{n+1}}{n+1}+c
		\\&=
			-\sum_{n=1}^\infty 5^{-n} \frac{x^{n}}{n}+c
\end{align*}$$

$$\begin{align*}
	\lim_{n\to\infty} \left| 5^{-n} \frac{x^{n}}{n} \right|
	&=
		\lim_{n\to\infty} \left| \frac{
			5^{-n-1} \frac{x^{n+1}}{n+1} 
		}{
			5^{-n} \frac{x^{n}}{n} 
		} \right|
	\\&=
		\lim_{n\to\infty} \left|
			5^{-1} \frac{xn}{n+1} 
		\right|
	\\&=
		|5^{-1}x| < 1
	\\&\equiv
		-5<x<5
\end{align*}$$

Then the radius of convergence is 5.
Then $x=0$ is in the interval of convergence, so sub $x=0$.
$$\begin{align*}
	\ln(5-0)
	&=
		\sum_{n=1}^\infty 5^{-n} \frac{0^{n}}{n}+c
	\\&=
		0+c
	\\ \ln 5 &= c
\end{align*}$$
$\therefore$ the power series representation is 
$$
	\sum_{n=1}^\infty \frac{x^{n}}{5^n n}+\ln 5
$$
![[Pasted image 20220213132110.png]]
$$\begin{align*}
	\int \frac{t}{1-t^8}\ dt
	&=
		\int \sum_{n=0}^\infty
		t (t^8)^n
	\\&=
		\int \sum_{n=0}^\infty
		t^{8n+1}
	\\&=
		\sum_{n=0}^\infty
		\frac{t^{8n+2}}{8n+2} + c
\end{align*}$$
$R=1$

![[Pasted image 20220213135253.png]]

*a)*
$$\begin{align*}
	\sum_{n=1}^\infty n x^{n-1}
	&=
		\frac d {dx} \int \sum_{n=1}^\infty nx^{n-1}
	\\&=
		\frac d {dx} \left( \sum_{n=1}^\infty x^n + c \right)
	\\&=
		\frac d {dx} \left( \frac 1 {1-x} - 1 + c \right)
	\\&=
		\frac 1 {(1-x)^2}
\end{align*}$$
*b)*
	*i)*
$$\begin{align*}
	\sum_{n=1}^\infty n x^n
	&=
		x \sum_{n=1}^\infty n x^{n-1}
	\\&=
		\frac x {(1-x)^2}
\end{align*}$$
	*ii)*
$$\begin{align*}
	\sum_{n=1}^\infty \frac n {2^n}
	&=
		\frac 1 2 \sum_{n=1}^\infty
		n \left( \frac 1 2 \right)^{n-1}
	\\&=
		\frac{\frac 1 2}{\left( 1 - \frac 1 2 \right)^2}
	\\&=
		2
\end{align*}$$
*c)*
	*i)*
$$\begin{align*}
	&\sum_{n=2}^\infty n(n-1)x^n
	\\&=
		\frac d {dx} \int \sum_{n=2}^\infty
		n(n-1)x^n\ dx
	\\&=
		x^2 \frac d {dx} \int \sum_{n=2}^\infty
		n(n-1)x^{n-2}\ dx
	\\&=
		x^2 \frac d {dx} \left( \sum_{n=2}^\infty
			n x^{n-1} + c
		\right)
	\\&=
		x^2 \frac d {dx} \frac d {dx} \left( \int
			\sum_{n=2}^\infty
			n x^{n-1} + c
		\ dx \right)
	\\&=
		x^2 \frac d {dx} \frac d {dx} \left(
			\sum_{n=2}^\infty
			x^n + cx + d
		\right)
	\\&=
		x^2 \frac d {dx} \frac d {dx} \left(
			\sum_{n=2}^\infty
			x^n + (-1 + 1) + (-x + x) + cx + d
		\right)
	\\&=
		x^2 \frac d {dx} \frac d {dx} \left(
			\sum_{n=0}^\infty
			x^n - 1 - x + cx + d
		\right)
	\\&=
		x^2 \frac d {dx} \frac d {dx} \left(
			\frac 1 {1 - x} - 1 - x + cx + d
		\right)
	\\&=
		x^2 \frac d {dx} \left(
			\frac 1 {(1 - x)^2} - x + cx
		\right)
	\\&=
		x^2 \left(
			\frac 2 {(1 - x)^3}
		\right)
	\\&=
		\frac{2x^2}{(1 - x)^3}
\end{align*}$$
	*ii)*
$$\begin{align*}
	&\sum_{n=2}^\infty \frac{n^2-n}{2^n}
	\\&=
		\sum_{n=2}^\infty \frac{n(n-1)}{2^n}
	\\&=
		\frac{2 \left( \frac 1 2 \right)^2}{
			\left( 1 - \frac 1 2 \right)^3
		}
	\\&=
		4
\end{align*}$$
	*iii)*
$$\begin{align*}
	&\sum_{n=1}^\infty \frac{n^2}{2^n}
	\\&=
		\sum_{n=1}^\infty \left(
			\frac{n^2}{2^n}
			- \frac{n}{2^n} + \frac{n}{2^n}
		\right)
	\\&=
		\sum_{n=2}^\infty \frac{n^2 - n}{2^n} 
		+ \sum_{n=1}^\infty \frac{n}{2^n}
	\\&=
		4 + 2
	\\&=
		6
\end{align*}$$

$$\begin{align*}
	\ln(5-x)
		&= \int \frac d {dx} \ln(5-x)\ dx \\
		&= -\int \frac {1}{5-x}\ dx\\
		&= -\int \frac 1 5 \frac {1}{1-\frac x 5}\ dx \\
	&= 
		-\int 
			\sum_{n=0}^\infty
				\frac 1 5 (\frac x 5)^n
		\ dx \\
	&= 
		-\int 
			\sum_{n=0}^\infty
				(\frac 1 5)^{n+1} x^n
		\ dx \\
	&= 
		-\int 
			\sum_{n=0}^\infty
				5^{-n-1} x^n
		\ dx \\
	\ln(5-x) &= 
			-\sum_{n=0}^\infty
				\frac{5^{-n-1}}{n+1} x^{n+1} + c
			\\
	\ln(5) &= 
			-\sum_{n=0}^\infty
				\frac{5^{-n-1}}{n+1} (0)^{n+1} + c
			\\
	\ln(5) &= c
			\\
	\ln(5-x) &= 
			-\sum_{n=0}^\infty
				\frac{5^{-n-1}}{n+1} x^{n+1} + \ln 5
			\\
\end{align*}$$
