# 14.2
![[Pasted image 20220326083156.png]]

![[Pasted image 20220326083224.png]]
56

![[Pasted image 20220326083323.png]]
$\pi/2$

![[Pasted image 20220326083536.png]]
![[Pasted image 20220326083529.png]]
$$y = 0 \Rightarrow lim = 0$$
$$x = 0 \Rightarrow lim = 1$$

![[Pasted image 20220326084026.png]]
$$y = x \Rightarrow lim = \frac 1 2$$
$$y = 0 \Rightarrow lim = 0$$

![[Pasted image 20220326084237.png]]
$$y = x \Rightarrow \lim = 1$$
$$y = 0 \Rightarrow \lim = 0$$

![[Pasted image 20220326084401.png]]
$$y = 0 \Rightarrow \lim = 0$$
$$x = y^2 \Rightarrow \lim = \frac 1 2$$

![[Pasted image 20220326084852.png]]
$$\begin{align*}
	\frac{2x^2}{\sqrt{2x^2 + 1} - 1} \\
	\frac{2x^2(\sqrt{2x^2 + 1} + 1)}{2x^2 + 1 - 1} \\
	\sqrt{2x^2 + 1} + 1 = 2
\end{align*}$$

$$\begin{align*}
	0 < \sqrt{x^2 + y^2} < \delta \\
	|\frac{x^2 + y^2}{\sqrt{x^2 + y^2 + 1} - 1} - 2| < \epsilon \\
\end{align*}$$

![[Pasted image 20220326090556.png]]

The functions $xy$ and $1 + e^{x-y}$ are continuous everywhere with $1 + e^{x-y} \ne 0$ so ye.

![[Pasted image 20220326090840.png]]
$1 + x^2 + y^2$ continuous everywhere, $1 - x^2 - y^2 = 0$ when $1 - (x^2 + y^2) = 0 \Rightarrow (1 - \sqrt{x^2 + y^2})(1 + \sqrt{x^2 + y^2})$ so when $1 - \sqrt{x^2 + y^2} = 0$. 

![[Pasted image 20220326091235.png]]
Continuous on its domain, when $x \ge 0$ and $1 - x^2 - y^2 \ge 0 \Rightarrow 1 \ge x^2 + y^2$  and $x \ge 0$.

![[Pasted image 20220326091432.png]]
For $(x, y) \ne (0, 0)$ it's a rational function. Then,

$$\begin{align*}
	0 < \sqrt{x^2 + y^2} < \delta \\
	|\frac{x^2 y^3}{2x^2 + y^2} - 1| < \epsilon \\
	2x^2 + y^2 \ge x^2 \\
	1 \ge \frac{x^2}{2x^2 + y^2} \\
	|\frac{x^2y^3}{2x^2 + y^2}| \le |y^3|
\end{align*}$$

As $y \to 0$, we have by squeeze theorem that $f(x, y) \to 0$.