# 8.2 Practice
![[Pasted image 20220219160631.png]]
![[Pasted image 20220219160646.png]]
*a)*
$$\begin{align*}
	y' &= \frac d {dx} \sqrt[3]{x} \\
	&= \frac 1 3 x^{-\frac 2 3} \\

	A &= \int_1^8 2 \pi \sqrt[3]{x} \sqrt{1+\left(\frac 1 3 x^{-\frac 2 3}\right)^2} dx
\end{align*}$$

*b)*
$$\begin{align*}
	y &= \sqrt[3] x \\
	y^3 &= x \\
	x' &= \frac d {dy} y^3 \\
	x' &= 3y^2 \\

	A &= \int_1^2 2 \pi y^3 \sqrt{
		1 + (3y^2)^2
	}\ dy \\
	&= \int_1^2 2 \pi y \sqrt{
		1 + 9y^4
	}\ dy
\end{align*}$$

![[Pasted image 20220219161551.png]]
*a)*
$$\begin{align*}
	y &= \frac 4 x \\
	y' &= \frac d {dx} \frac 4 x \\
	&= -4x^{-2} \\

	A &= 
		\int_1^8 2 \pi x \sqrt{
			1 + (-4x^{-2})^2 
		}\ dx \\
	&= 
		\int_1^8 2 \pi x \sqrt{
			1 + 16x^{-4}
		}\ dx \\
\end{align*}$$

*b)*
$$\begin{align*}
	x &= \frac 4 y \\
	x' &= \frac d {dy} \frac 4 y \\
	&= -4y^{-2} \\

	A &=
		\int_4^{\frac 1 2} 2 \pi \frac 4 y \sqrt{
			1 + (-4y^{-2})
		}\ dy
\end{align*}$$

![[Pasted image 20220219163114.png]]
$$\begin{align*}
	y &= \sqrt{x+1} \\
	y' &= \frac 1 2 (x+1)^{-\frac 1 2} \\

	A &=
		\int_0^3 2 \pi \sqrt{x+1} \sqrt{
		1 + \left(\frac 1 2 (x+1)^{-\frac 1 2}\right)^2
	}\ dx \\
	&=
	\int_0^3 2 \pi \sqrt{x+1} \sqrt{
		1 + \frac 1 4 (x+1)^{-1}
	}\ dx \\
	&=
	\int_0^3 2 \pi \sqrt{x+1} (x+1)^{-\frac 1 2} \sqrt{
		x+1 + \frac 1 4
	}\ dx \\
	&=
	\int_0^3 2 \pi \sqrt{
		x + \frac 5 4
	}\ dx \\
	&=
		2 \pi \left( \frac 2 3 \left(x + \frac 5 4 \right)^{\frac 3 2}\right) \Big|_0^3 \\
	&=
		\frac 4 3 \pi \left(\left( \frac{17}{4}\right)^{\frac 3 2} - \left( \frac{5}{4}\right)^{\frac 3 2} \right) \\
\end{align*}$$

![[Pasted image 20220219171043.png]]
$$\begin{align*}
	y &= \tfrac{x^3}{6} + \tfrac{1}{2x} \\
	y' &= \frac d {dx} (\tfrac{x^3}{6} + \tfrac{1}{2x}) \\
	&= \tfrac{x^2}{2} - \tfrac{1}{2x^{2}} \\

	A &= 
		\int_{\frac 1 2}^1 2 \pi (\tfrac{x^3}{6} + \tfrac{1}{2x}) \sqrt{
			1 + (\tfrac{x^2}{2} - \tfrac{1}{2x^{2}})^2
		}\ dx \\
	&= 
		\int_{\frac 1 2}^1 2 \pi (\tfrac{x^4+3}{6x}) \sqrt{
			1 + (\tfrac{x^4-1}{2x^{2}})^2
		}\ dx \\
	&= 
		\int_{\frac 1 2}^1 2 \pi (\tfrac{x^4+3}{6x}) \sqrt{
			1 + \tfrac{x^8-2x^4+1}{4x^{4}}
		}\ dx \\
	&= 
		\int_{\frac 1 2}^1 2 \pi (\tfrac{x^4+3}{6x}) \sqrt{
			\tfrac{x^8+2x^4+1}{4x^{4}}
		}\ dx \\
	&= 
		\int_{\frac 1 2}^1 2 \pi 
			(\tfrac{x^4+3}{6x}) 
			(\tfrac{x^4+1}{2x^{2}})
		\ dx\\
	&= 
		\int_{\frac 1 2}^1 \pi 
			\frac{x^8+4x^4+3}{6x^3}
		\ dx\\
	&= 
		\int_{\frac 1 2}^1 \pi 
			(\tfrac 1 6 x^5 + \tfrac 2 3 x + \tfrac 1 {2x^3})
		\ dx\\
	&= 
		\pi (\tfrac 1 {36} x^6 + \tfrac 1 3 x^2 - \tfrac 1 4 x^{-2}) \Big|_{\frac 1 2}^1 \\
	&=
		\pi (\tfrac 1 9 + \tfrac{2111}{2304}) \\
	&=
		\pi \frac{263}{256}
\end{align*}$$

![[Pasted image 20220219174810.png]]
$$\begin{align*}
	x' &=
		\frac d {dx} \frac 1 3 \left(
			y^2+2
		\right)^{\frac 3 2}
	\\&=
		\frac 1 2 \left(
			y^2+2
		\right)^{\frac 1 2}(2y)
	\\&=
		\left(
			y^2+2
		\right)^{\frac 1 2}y
\end{align*}$$

$$\begin{align*}
	A &=
		\int_1^2
			2 \pi \frac 1 3 y 
			\sqrt{
				1 + ((y^2+2)^{\frac 1 2}y)^2
			}
		\ dy \\
	&=
		\int_1^2
			\pi \frac 2 3 y
			\sqrt{
				1 + (y^2+2)y^2
			}
		\ dy \\
	&=
		\int_1^2
			\pi \frac 2 3 y
			\sqrt{
				(y^2+1)^2
			}
		\ dy \\
	&=
		\int_1^2
			\pi \frac 2 3 y
				(y^2+1)
		\ dy \\
	&=
		\pi \frac 2 3
		\int_1^2
				y^3+y
		\ dy \\
	&=
		\frac 2 3 \pi \left(\frac 1 4 y^4 + \frac 1 2 y^2 \right) \Big|_1^2 \\
	&=
		\frac 2 3 \pi \left( 6 + \frac 3 4 \right) \\
	&=
		\frac 9 2 \pi
\end{align*}$$

![[Pasted image 20220219181836.png]]
$$\begin{align*}
	y &= \frac 1 3 x^{\frac 3 2} \\
	y' &= \frac d {dx} \frac 1 3 x^{\frac 3 2} \\
	&= \frac 1 2 x^{\frac 1 2} \\
\end{align*}$$

$$\begin{align*}
	A &=
		\int_0^{12} 2 \pi x
		\sqrt{
			1 + \left( \frac 1 2 x^{\frac 1 2} \right)^2
		}
		\ dx
	\\&=
		\int_0^{12} 2 \pi x
		\sqrt{
			1 + \frac 1 4 x
		}
		\ dx
\end{align*}$$

Let $u=1+\frac 1 4 x$, then $4du = dx$

$$\begin{align*}
	&=
		\int_1^{4} 2 \cdot 4 \pi 4\left(u - 1\right)
		\sqrt{
			u
		}
		\ du
	\\&=
		\int_1^{4} 32 \pi \left(
			u^{\frac 3 2} - u^{\frac 1 2}
		\right)
		\ du
	\\&=
		32 \pi \left(
			\frac 2 5 u^{\frac 5 2} 
			- \frac 2 3 u^{\frac 3 2} 
		\right) \Big|^4_1
	\\&=
		32 \pi \left(
			\frac{112}{15}
			+ \frac 4 {15}
		\right)
	\\&=
		\frac{3712}{15}
\end{align*}$$

![[Pasted image 20220219185533.png]]
$$\begin{align*}
	y^{\frac 2 3} &= 1 - x^{\frac 2 3} \\
	\frac d {dx} y &=
		\frac d {dx}
		\left(1 - x^{\frac 2 3}\right)^{\frac 3 2} \\
	y' &=
		\frac 3 2 \left(1 - x^{\frac 2 3}\right)^{\frac 1 2}
		\cdot
		-\frac 2 3x^{-\frac 1 3}\\
	&=
		-\left(1 - x^{\frac 2 3}\right)^{\frac 1 2}
		x^{-\frac 1 3}\\
	&=
		-\left(x^{-\frac 2 3} - 1\right)^{\frac 1 2}
\end{align*}$$

When $y = 0$, $x = 1$ and when $y = 1, x=0$.

$$\begin{align*}
	A &= 
		\int_0^1 2 \pi x 
		\sqrt{
			1 + 
			\left(-\left(x^{-\frac 2 3} - 1\right)^{\frac 1 2}\right)^2
		}
	\\&=
		\int_0^1 2 \pi x 
		\sqrt{
			1 + 
			\left(x^{-\frac 2 3} - 1\right)
		}
	\\&=
		\int_0^1 2 \pi x 
		x^{-\frac 1 3}
	\\&=
		\int_0^1 2 \pi x^{\frac 2 3}
	\\&=
		2 \pi \frac 3 5 x^{\frac 5 3} \Big|_0^1
	\\&=
		\frac 6 5 \pi
\end{align*}$$

![[Pasted image 20220219190839.png]]
$$\begin{align*}
	y &= \frac 1 x \\
	y' &= -\frac 1 {x^2} \\
\end{align*}$$

$$\begin{align*}
	A &=
		\int_1^\infty 2 \pi
		\left(\frac 1 x\right)
		\sqrt{
			1 + \left(
				-\frac 1 {x^2}
			\right)^2
		}
		\ dx
	\\&=
		\int_1^\infty 2 \pi
		\left(\frac 1 x\right)
		\sqrt{
			\frac{x^4 + 1}{x^4}
		}
		\ dx
	\\&=
		\int_1^\infty 2 \pi
		\left(\frac 1 {x^3}\right)
		\sqrt{
			x^4 + 1
		}
		\ dx
\end{align*}$$

Let $u = x^4+1$. Then, $\frac 1 {4x^3} du = dx$.

$$\begin{align*}
	&=
		\int_1^\infty \frac 1 2 \pi
		\sqrt{
			u
		}
		\ dx
	\\&=
		\pi \frac 1 3 u^{\frac 3 2} \Big|_1^\infty
	\\&=
		\infty
\end{align*}$$