# 9.3
![[Pasted image 20220304110907.png]]
![[Pasted image 20220304110951.png]]
*Notice*: $p=-1$ is a solution.

*Case $p \neq -1$*
$$\begin{align*}
	\frac{dp}{dt}
	&=
		t^2p-p+t^2-1 \\
	\frac{dp}{dt}
	&=
		(p+1)(t^2-1) \\
	\int \frac 1 {p+1}\ dp 
	&=
		\int t^2-1\ dt \\
	\ln |p+1|
	&=
		\frac 1 3 t^3 - t + c \\
	\tag{$c$ can be <0 or >0}
	|p+1|
	&=
		c e^{\frac 1 3 t^3 - t} \\
	p+1
	&=
		c e^{\frac 1 3 t^3 - t} \\
	p
	&=
		c e^{\frac 1 3 t^3 - t} - 1 \\
\end{align*}$$

![[Pasted image 20220304112702.png]]

*Notice:* no constant solutions for the derivative.

$$\begin{align*}
	\frac{dy}{dx}
	&=
		\frac{
			x \ln x
		}{
			y (1 + \sqrt{3 + y^2})
		} \\
	\int y (1 + \sqrt{3 + y^2})\ dy
	&=
		\int x \ln x \ dx \\
\end{align*}$$

$$\begin{align*}
	a &= 3 + y^2
	&\implies
	&&\frac 1 2 \ da &= y \ dy \\
	
	u &= \ln x
	&\implies
	&&du &= \frac 1 x \ dx \\
	
	dv &= x \ dx
	&\implies
	&&v &= \frac 1 2 x^2
\end{align*}$$

$$\begin{align*}
	\frac 1 2 \int 1 + \sqrt a \ da
	&=
		\frac 1 2 x^2 \ln x
		-
		\int \frac 1 2 x^2 \frac 1x \ dx \\
	
	\frac 1 2 \left( 
		a + \frac 2 3 a^{\frac 3 2}
	\right)
	&=
		\frac 1 2 x^2 \ln x
		-
		\frac 1 2 \left( \frac 1 2 x^2 \right) + c \\
		
	\frac 1 2 \left( 
		3 + y^2 + \frac 2 3 (3 + y^2)^{\frac 3 2}
	\right)
	&=
		\frac 1 2 x^2 \ln x
		-
		\frac 1 2 \left( \frac 1 2 x^2 \right) + c \\
		
	\frac 1 2 y^2 + \frac 1 3 (3 + y^2)^{\frac 3 2}
	&=
		\frac 1 2 x^2 \ln x
		-
		\frac 1 2 \left( \frac 1 2 x^2 \right) + c \\
	
	y(1) = 1 
	\implies
	\frac 1 2 (1)^2 + \frac 1 3 (3 + (1)^2)^{\frac 3 2}
	&=
		\frac 1 2 (1)^2 \ln (1)
		-
		\frac 1 2 \left( \frac 1 2 (1)^2 \right) + c \\
	
	\frac{19}{6}
	&=
		-\frac 1 4 + c \\
	
	c &= \frac{41}{12} \\
	
	\therefore 
	\frac 1 2 y^2 + \frac 1 3 (3 + y^2)^{\frac 3 2}
	&=
		\frac 1 2 x^2 \ln x
		-
		\frac 1 4 x^2 + \frac{41}{12} \\
\end{align*}$$

![[Pasted image 20220304115629.png]]
$$\begin{align*}
	\frac{dy}{dx}
	&=
		\frac x y \\
	
	\int y \ dy
	&=
		\int x \ dx \\
	
	\frac 1 2 y^2
	&=
		\frac 1 2 x^2 + c \\
	
	y &= \pm \sqrt{x^2 + c} \\
	
	y(0) = 2 \implies
	2 &= \pm \sqrt{(0)^2 + c} \\
	2 &= \sqrt{(0)^2 + c} \\
	c &= 4 \\
	\\
	\therefore y &= \sqrt{x^2+4}
\end{align*}$$

![[Pasted image 20220304120503.png]]
$$\begin{align*}
	\frac{df}{dx} &= x(f(x) - 1) \\
	
	\int \frac{1}{f(x) - 1} \ df
	&=
		\int x \ dx \\
	
	\ln|f(x) - 1| &= \frac 1 2 x^2 + c \\
	
	f(x) &= ce^{\frac 1 2 x^2} + 1 \\
	
	f(0) = 2 \implies
	2 &= ce^{\frac 1 2 0^2} + 1 \\
	
	c &= 1 \\
	
	\therefore f(x) &= e^{\frac 12 x^2} + 1
\end{align*}$$

![[Pasted image 20220304121416.png]]
$$\begin{align*}
	\frac d {dx} (x^2 + 2y^2) &= \frac d {dx} k^2 \\
	
	2x + 4yy' &= 0 \\
	
	y' &=
		\frac{x}{2y} \\
	
	\implies
	y' &= \frac{2y}{x} \\
	
	\int \frac 1 {2y} \ dy
	&=
		\int \frac 1 x \ dx \\
	
	\frac 1 2 \ln |y| &= \ln|x| + c \\
	
	\ln |y| &= 2 \ln|x| + c \\
	
	y &= ce^{2 \ln|x|} \\
	
	y &= cx^{2} \\
\end{align*}$$

![[Pasted image 20220304122538.png]]
$$\begin{align*}
	\int \frac 1 {M - P} \ dP
	&=
		\int k \ dt \\
	
	- \ln |P - M|
	&=
	kt + c \\
		
	|P - M|
	&=
		c e^{- kt} \\
		
	P
	&=
		c e^{- kt} + M \\
		
	\lim_{t \to \infty} P
	&=
		\lim_{t \to \infty} \left(
			c e^{- kt} + M \\
		\right) \\
		
	\lim_{t \to \infty} P
	&=
		M
\end{align*}$$

![[Pasted image 20220304124322.png]]
*a)*
Let $y$ be the concentration of salt after $t$ minutes.

$$\begin{align*}
	\frac{dy}{dt}
	&=
		- \frac{10y(t)}{1000} \\
		
	\int \frac 1 y \ dy
	&=
		-\frac 1 {100} \int \ dt \\
		
	\ln|y| &= -\frac 1 {100} t + c \\
	
	y &= c e^{-\frac 1 {100} t} \\
	
	y(0) = 15 \implies
	15 &= c e^{-\frac 1 {100} (0)} \\
	c &= 15 \\
	
	\therefore y &= 15 e^{-\frac 1 {100} t} \text{ kg} \\
\end{align*}$$

*b)*
$$\begin{align*}
	y(20) &= 15 e^{-\frac 1 {100} (20)} \\
	&= 15 e^{-\frac 1 5} \text{ kg} \\
	&\approx 12.28 \text{ kg}
\end{align*}$$

