# 9.5
![[Pasted image 20220310130815.png]]

![[Pasted image 20220310131644.png]]
$$\begin{align*}
	e^x(y' + y) &= e^xx \\
	\frac d {dx} (e^xy) &= e^xx \\
	e^x y &= \int e^x x \ dx \\
	e^x y &= e^x x  - \int e^x \ dx \\
	e^x y &= e^x x  - e^x + c\\
	y &= x - 1 + \frac c {e^x}
\end{align*}$$

![[Pasted image 20220310132546.png]]
$$\begin{align*}
	xy' + y &= \sqrt x \\
	(xy)' &= \sqrt x \\
	xy &= \int \sqrt x \ dx \\
	xy &= \frac 2 3 x^{3/2} + c \\
	y &= \frac 2 3 x^{1/2} + \frac c x \\
\end{align*}$$

![[Pasted image 20220310133255.png]]
$$\begin{align*}
	y'x^{-2} - 2x^{-3}y &= x^{-1} \\
	(x^{-2}y)' &= x^{-1} \\
	x^{-2}y &= \int x^{-1} \ dx \\
	x^{-2}y &= \ln |x| + c \\
	y &= \ln|x|x^2 + cx^2 \\
\end{align*}$$

![[Pasted image 20220310134132.png]]
$$\begin{align*}
	t^3y' + 3t^2y &= t \sqrt{1 + t^2} \\
	(t^3y)' &= t \sqrt{1 + t^2} \\
	t^3y &= \int t \sqrt{1 + t^2} \ dt \\
	t^3y &= \frac 1 3 (1 + t^2)^{3 / 2} + c\\
	y &= \frac{\frac 1 3 (1 + t^2)^{3 / 2} +  c}{t^3} \ dt \\
\end{align*}$$

![[Pasted image 20220310145755.png]]
$$\begin{align*}
	(x^2y)' &= \ln x \\
	x^2y &= \int \ln x \ dx \\
	x^2y &= x \ln x - \int dx \\
	x^2y &= x \ln x - x + c \\
	y &= x^{-1} \ln x - x^{-1} + cx^{-2} \\
	y(1) = 2 \Rightarrow
	2 &= 1^{-1} \ln 1 - 1^{-1} + c(1)^{-2} \\
	c &= 3 \\
	y &= x^{-1} \ln x - x^{-1} + 3x^{-2} \\
\end{align*}$$

![[Pasted image 20220310152200.png]]
![[Pasted image 20220310152208.png]]
$$\begin{align*}
	5 Q' + \frac 1 {0.05}Q &= 60 \\
	Q' + 4Q &= 12 \\
	e^{4t}Q' + 4e^{4t}Q &= 12e^{4t} \\
	(e^{4t}Q)' &= 12e^{4t} \\
	e^{4t}Q &= 12 \int e^{4t} \ dt \\
	e^{4t}Q &= 12 (\frac 1 4 e^{4t}) + c \\
	Q &= 3 + \frac c {e^{4t}} \\
	Q(0) = 0 \Rightarrow
	0 &= 3 + \frac c {e^{4(0)}} \\
	c &= -3 \\
	Q &= 3 + \frac{-3}{e^{4t}} \\
	Q' &= \frac Q {dt} \left( 3 + \frac{-3}{e^{4t}} \right) \\
	I &= -12e^{-4t}
\end{align*}$$

![[Pasted image 20220310153542.png]]
![[Pasted image 20220310153556.png]]
$$\begin{align*}
	y' &= 2 - \frac{3y}{100+2t} \\
	y' + \frac{3y}{100+2t} &= 2 \\
	\\
	\int \frac 3 {100+2t} \ dt
	&=
		\frac 3 2 \ln|100+2t| + c \\
	\\
	e^{\frac 3 2 \ln|100+2t|}
	&=
		|100+2t|^{\frac 3 2} \\
	\\
	|100+2t|^{\frac 3 2}y' + |100+2t|^{\frac 3 2}\frac{3y}{100+2t} &= 2|100+2t|^{\frac 3 2} \\
	(|100+2t|^{3/2}y)' &= 2|100+2t|^{\frac 3 2} \\
	|100+2t|^{3/2}y &= \int 2|100+2t|^{\frac 3 2} \ dt \\
	|100+2t|^{3/2}y &= \frac 2 5 |100+2t|^{\frac 5 2} + c \\
	y &= \frac 2 5 |100+2t| + c|100+2t|^{-\frac 3 2} \\
	y(0) = 0 \Rightarrow 
	0 &= \frac 2 5 |100+2(0)| + c|100+2(0)|^{-\frac 3 2} \\
	-40 &= c|100|^{-\frac 3 2} \\
	-40000 &= c \\
	y &= \frac 2 5 |100+2t| - 40000|100+2t|^{-\frac 3 2} \\
	y(20) &= \frac 2 5 |100+2(20)| - 40000|100+2(20)|^{-\frac 3 2} \\
	&\approx 31.85 \text{ kg}
\end{align*}$$