# 1)
1) $b+2$
2) $b + 2 + y \cdot (b+2)$
3) $x \cdot y + (x \cdot y \cdot 2)$
4) $x + x \cdot 2$
5) $x + y + (x + y) \cdot y + (x + y) \cdot y \cdot z$

# 2)
1) $b+2$
2) $x + y \cdot (b+2)$
3) $(b+2) + (x+2) \cdot (b+2)$
4) $(x \cdot y + x \cdot y \cdot 2)$
5) $(x \cdot y + x \cdot y \cdot 2)$
6) $(y + y \cdot x +y \cdot x \cdot z)$

# 4)
Suppose $E[z:=X]=E[z:=Y]$ is true in every state for every expression $E$. Then, $E : z$  would be such a valid expression, such that $E[z:=X]=E[z:=Y] \equiv z[z:=X]=z[z:=Y] \equiv X = Y$ . So $X = Y$ is true in every state.

# 5)
proved in *4)* that $E[z:=X]=E[z:=Y] \Leftrightarrow X=Y$ so replace it and then we get $\frac{Z=X, Z=Y}{X=Y}$ and bam the transitivity rule proven.

# 6)
$$\begin{matrix*}
	\dfrac{x < y \lor x \ge y}{1<y \lor 1 \ge y} &&
	\dfrac{x < y \lor x \ge y}{2<y \lor 2 \ge y} &&
	\dfrac{x < y \lor x \ge y}{3<y \lor 3 \ge y} &&
\end{matrix*}$$

# 7)
1) $4\cdot(x+2)+y$
2) $x + 5 \cdot w$
3) $3 \cdot y + 3 \cdot x + 1$
4) $y + y$, $y + x$, $x + y$, $x + x$
5) $(y+1) \cdot x + (y + 1) \cdot y$, $7 \cdot x + 7 \cdot y$ , $(y + 1) \cdot x + 7 \cdot y$, $y \cdot x + (y + 1) \cdot y$

# 8)
1) $b + c + y + w$
2) $x + y + w$
3) $x \cdot (x + y)$
4) $(x + y) \cdot x \cdot y$
5) $(y + x) \cdot q \cdot (y + x)$

# 9)
$E: (x + y) \cdot z$, $X = Y \equiv x + y = y + x$

# 11)
