![[Pasted image 20220922093241.png]]
- *Monotonicity* if $(x \Rightarrow y) \Rightarrow (f(x) \Rightarrow f(y))$


> [!example] Prove (4.2)
> ![[Pasted image 20220922094540.png]]
> ![[Pasted image 20220922094556.png]]
> Starting with the consequence, we were forced to use $\Leftarrow$. Starting with the antecedent, we can use $\Rightarrow$.

```ad-note
title: Deduction Theorem

Suppose adding $P_1, \dots, P_n$ as axioms to propositional logic, with the variables of the $P_i$ considered to be constants, allows $Q$ to be proved. Then $P_1 \land \dots \land P_n \Rightarrow Q$ is a theorem.
```


