# Bayes' Theorem
Suppose that $E$ and $F$ are events from sample space $S$ such that $p(E) \neq 0$ and $p(F) \ne 0$. Then:

$$
	p(F \mid E) 
	=
		\frac{p(E \mid F)p(F)}{
			p(E \mid F) p(F)
			+ p(E \mid \overline F) p(\overline F)
		}
$$

### Proof
*Recall*: $p(E \mid F) = \frac{p(E \cap F)}{p(F)}$

Thus,
$$
	p(E \mid F) p(F) = p(E \cap F),\
	p(F \mid E) p(E) = p(E \cap F)
$$
Equating both formulas,
$$p(E \mid F) p(F) = p(F \mid E) p(E)$$
And solving for $p(E \mid F)$ and for $p(F \mid E)$:
$$p(E \mid F) = \frac{p(F \mid E) p(E)}{p(F)}$$

##### Observe
$$\begin{align*}
	p(E) &= p(E \cap S)
	\\&= p(E \cap (F \cup \overline F))
	\\&= p((E \cap F) \cup (E \cap \overline F))
	\\&= 
		p(E \cap F) + p(E \cap \overline F)
		- p(E \cap F \cap E \cap \overline F)
	\\&= 
		p(E \cap F) + p(E \cap \overline F) - p(\emptyset)
	\\&= 
		p(E \cap F) + p(E \cap \overline F)
	\\&= p(E \mid F) p(F) + p(E \mid \overline F) p(\overline F)
\end{align*}$$

Hence,
$$
	p(E \mid F) = \frac{
		p(E \mid F) p(F)
	}{
		p(E \mid F) p(F)
		+ p(E \mid \overline F) p(\overline F)
	}
$$

# Generalized Bayes' Theorem
Suppose that $E$ is an event from a sample space $S$ and that $F_1, F_2, \dots, F_n$ are *mutually exclusive* events such that $bigcup_i^n F_i = S$.

Assume that $p(E) \ne 0$ for $i = 1, 2, \dots, n$. Then,
$$
	p(F_j \mid E)
	=
		\frac{
			p(E \mid F_j) p(F_j)
		}{
			\sum_{i=1}^{n}
			p(E \mid F_i) p(F_i)
		}
$$