# Multivariable Chain Rule
How do we differentiate $z = f(x, y)$ when $x$ and $y$ are functions of other variables?

### Example
Let $x = g(t), y = h(t) \rightarrow z = f(g(t), h(t))$.
- Then $z$ is a function of $t$.
- Want to find $\frac{dz}{dt}$, so differentiate along all branches from $z$ to $t$.
- Multiply along branches, add between branches

![[Pasted image 20220407134758.png|250]]

$$\begin{align*}
	\frac{dz}{dt} &=
		\frac{\partial f}{\partial x} \frac{dx}{dt}
		+ \frac{\partial f}{\partial y} \frac{dy}{dt}
	\\
	z &= f(x, y) = xy^3 - x^2 y \\
	x &= t^2 + 1 \\
	y &= t^2 - 1 \\
	\\
	\frac{d}{dt} \left( xy^3 - x^2 y \right)
	&=
		(y^3 - 2x y)(2t) + (3xy^2 - x^2)(2t) \\
	&= 2t(
		((t^2 - 1)^3 - 2(t^2 + 1)(t^2 - 1))
		+
		3(t^2 + 1)(t^2 - 1)^2 - (t^2 + 1)^2
	)
\end{align*}$$

### Example
Let $x = g(s, t), y = h(s, t), z = f(x, y)$

$$\begin{align*}
	\frac{dz}{dt}
		&= \frac{\partial f}{\partial x} 
			\frac{\partial x}{\partial t}
		+
		\frac{\partial f}{\partial y}
			\frac{\partial y}{\partial t}
		\\
	\frac{dz}{ds}
		&= \frac{\partial f}{\partial x} 
			\frac{\partial x}{\partial s}
		+
		\frac{\partial f}{\partial y}
			\frac{\partial y}{\partial s}
\end{align*}$$

## Chain Rule: Case 1
![[Pasted image 20220407133706.png]]
- Basically like the product rule but with 2 variables.

![[Pasted image 20220407134033.png]]
![[Pasted image 20220407134218.png]]

## Application: Implicit Differentiation
One independent variable: $y$ depends on $x$.
- ***Implicit equation*** - something we can't solve for $y$ as a function of $x$.

$$F(x, y) = c$$
- $F(x, y)$ - Shift everything with $x$ or $y$ to the left side
- $c$ - Constant on the right

$$\begin{align*}
	\frac \partial {\partial x} F(x, y) &= \frac d {dx} c \\
	0 &=
		\frac{\partial F}{\partial x} + \frac{\partial F}{\partial y} \frac{dy}{dx} \\
	0 &=
		F_x + F_y \frac{dy}{dx} \\
	\frac{dy}{dx} &= -\frac{F_x}{F_y}
\end{align*}$$
- Formula for implicit differentiation with one variable.


